add new cca2Compliant

src/voteprivacy/contextCompHid.v
@@ -1,12 +1,13 @@
 Require Export auxDefs.
 Import ListNotations.
 
-Module Cxt.
+Module CxtCompHid.
 
 Definition CxtTwoVarsMsg: Type:= message -> message -> message.
 Definition CxtTwoVarsBol: Type:= message -> message -> Bool.
 
-Definition CxtListTwoVars: Type:= message -> message ->list message.
+Definition CxtListTwoVars: Type:= message -> message -> list message.
+
 
 Inductive IsContextMsg: CxtTwoVarsMsg -> Prop:=
 | CO: IsContextMsg (fun _ _ => O)
@@ -32,6 +33,15 @@ Inductive IsContextMsg: CxtTwoVarsMsg -> Prop:=
 | CV0 C1 (H1: IsContextMsg C1): IsContextMsg (fun (x: message) (y: message) => V0 (C1 x y))
 | CV1 C1 (H1: IsContextMsg C1): IsContextMsg (fun (x: message) (y: message) => V1 (C1 x y))
 | Cpubkey C1 (H1: IsContextMsg C1): IsContextMsg (fun (x: message) (y: message) => pubkey (C1 x y))
+(* Commitments *)
+| Ckc C1 (H1: IsContextMsg C1): IsContextMsg (fun (x: message) (y: message) => kc (C1 x y))
+| Ccomm C1 C2 (H1: IsContextMsg C1) (H2: IsContextMsg C2):
+  IsContextMsg (fun (x: message) (y: message) => comm (C1 x y) (C2 x y))
+| Copen C1 C2 C3 (H1: IsContextMsg C1) (H2: IsContextMsg C2) (H3: IsContextMsg C3):
+  IsContextMsg (fun (x: message) (y: message) => open (C1 x y) (C2 x y) (C3 x y))
+(* shuffling *)
+| Cshufle C1 C2 C3 (H1: IsContextMsg C1) (H2: IsContextMsg C2) (H3: IsContextMsg C3):
+  IsContextMsg (fun (x: message) (y: message) => shufl (C1 x y) (C2 x y) (C3 x y))
 (* Encryptions  *)
 | Cke C1 (H1: IsContextMsg C1): IsContextMsg (fun (x: message) (y: message) => ke (C1 x y))
 | Cre C1 (H1: IsContextMsg C1): IsContextMsg (fun (x: message) (y: message) => re (C1 x y))
@@ -91,18 +101,73 @@ Inductive IsContextOslist: CxtOslistTwoVars -> Prop :=
 | Cnil: IsContextOslist (fun (x: message) (y: message) => [ ])
 | Ccons C L (H1:IsContextOs C) (H2:IsContextOslist L): IsContextOslist (fun (x :message) (y: message) => (C x y)::(L x y)).
 
+(* Definition CxtMylist (n: nat) : Type := message -> message -> mylist n. *)
 
+(* Inductive IsContextMylist {n}: CxtMylist n -> Prop :=. *)
+  
+
+(* Axiom CxtListCxtMylist: forall {n} (l: mylist n), IsContextListMsg (fun (x: message) (y: message) => (toListm l)) -> IsContextMylist  (fun (x: message) (y: message) => l). *)
+                              
 Definition Test : CxtTwoVarsMsg:=  (fun (x: message) (y:message) => pair (V0 x) y).
 Definition TestList: CxtListTwoVars := (fun (x: message) (y: message) => [x; y]).
 Lemma TestContext: IsContextMsg Test.
 Proof. repeat constructor.
 Qed.
 
-Lemma TestContextList: IsContextListMsg TestList.
-                                    
+Definition contextPhi1:= (fun (x: message) (y: message) => let v0 := V0 (f (toListm phi0)) in
+      let v1 := V1 (f (toListm phi0)) in
+      (* Bothsides *)
+      let r0 := (r 1) in
+      let r1 := (r 2) in
+      let k0 := (kc (nonce 3)) in
+      let k1 := (kc (nonce 4)) in
+
+                                                                                             (* Left-side *)
+      let c00 := (comm v0 k0) in
+      let c11 := (comm v1 k1) in
+      let t := pubkey (f (toListm phi0)) in
+      let b00 := (bl x t r0) in
+      let b11 := (bl y t r1) in
+      (* let t0 := (((vk 0), (Mvar 5), sign (Mvar 5) (ssk 0) (sr 14)), ((vk 1), (Mvar 6), sign (Mvar 6) (ssk 1) (sr 15))) in *)
+      (* let t1 := (t0, f (cons t0 nil)) in *)
+      let t2 := (((vk 0), b00, sign b00 (ssk 0) (sr 14)), ((vk 1), b11, sign b11 (ssk 1) (sr 15))) in
+      let t3 := (t2, f (cons t2 nil)) in
+      (* let t2 := ({{ 5 := b00 }} ({{ 6:= b11 }} t0)) in *)
+      (* let t3  := ({{ 5 := b00 }} ({{ 6:= b11 }} t1)) in *)
+      let acc00 := (acc c00 t r0 t2) in
+      let acc11 := (acc c11 t r1 t3) in
+      let pv00 := (c00, ((ub c00 t r0 t2), (nonce 20))) in
+      let pv11 := (c11, ((ub c11 t r1 t3), (nonce 21))) in
+      let e00 := (enc (pv00, TWO) (pke 11) (er 7)) in
+      let e11 := (enc (pv11, TWO) (pke 11) (er 8)) in
+      let phi02:= [msg b00, msg b11, msg e00, msg e11] in
+      let fphi02:= f (toListm phi02) in
+      let s0 := (If (! (isin pv00 ((pi1 (d 1 fphi02)), ((pi1 (d 2 fphi02)), (pi1 (d 3 fphi02))))))
+                 then (shufl (pi1 (d 1 fphi02)) (pi1 (d 2 fphi02)) (pi1 (d 3 fphi02))) else O)in
+      let dv0 := (If (dist fphi02) & (pvchecks fphi02) then s0 else |_) in
+      let phi03:= phi02 ++[msg dv0] in
+      let fphi03 := f (toListm phi03) in
+      fphi03).
+                                                                                                            (*let l00 := (If (bnlcheck c00 (nonce 20) fphi03)
+                  then (enc ((label c00 fphi03), (k0, THREE)) (pke 11) (er 9)) else O) in
+      let l11 := (If (bnlcheck c11 (nonce 21) fphi03)
+                  then (enc ((label c11 fphi03), (k1, THREE)) (pke 11) (er 10)) else O) in
+      let phi05:= phi03++[msg l00, msg l11] in
+      let fphi05 := f (toListm phi05) in
+      let do0 := (If (dist fphi05) & (pochecks fphi05) & ((isink k0 fphi05) & (isink k1 fphi05)) (*or (! ((isink k0 fphi05)or (isink k1 fphi05))))*)
+                  then (sotrm fphi05) else |_) in
+      let t0s0 := (If acc00 & acc11 then ((e00, (e11, dv0)), (l00, (l11, do0))) else |_) in
+      f (toListm [msg b00, msg b11, msg t0s0])).
+ *)
+Lemma TestContextPhi1: IsContextMsg contextPhi1.
+Proof. repeat constructor.
+Qed.
+
+
+Lemma TestContextList: IsContextListMsg TestList.                                    
 Proof.
 repeat constructor.
 Qed.
 
 
-End Cxt.
+End CxtCompHid.
