src/voteprivacy/latestTactics.v
@@ -1,0 +1,804 @@
+(************************************************************************)
+(* Copyright (c) 2017-2018, Ajay Kumar Eeralla <ae266@mail.missouri.edu>*) 
+(************************************************************************)
+Require Export auxDefs.
+
+(* Module aux. *)
+(*   Export destructTerm. *)
+(*   Fixpoint submsg_bol pk r (t': message)(s: message) (b: Bool): Bool := *)
+(*     match b with *)
+(*     | eqb  b1 b2 =>  (eqb (submsg_bol pk r t' s b1) (submsg_bol pk r t' s b2)) *)
+(*     | eqm t1 t2 => (eqm (submsg_msg pk r t' s t1) (submsg_msg pk r t' s t2)) *)
+(*     | ifb_then_else_ t1 t2 t3 => (IF (submsg_bol pk r t' s t1) then (submsg_bol pk r t' s t2) else (submsg_bol pk r t' s t3)) *)
+(*     | ver t1 t2 t3 => ver (submsg_msg pk r t' s t1) (submsg_msg pk r t' s t2) (submsg_msg pk r t' s t3) *)
+(*     | bver t1 t2 t3 => bver (submsg_msg pk r t' s t1) (submsg_msg pk r t' s t2) (submsg_msg pk r t' s t3) *)
+(*     | acc t1 t2 t3 t4 => acc (submsg_msg pk r t' s t1) (submsg_msg pk r t' s t2) (submsg_msg pk r t' s t3) (submsg_msg pk r t' s t4) *)
+(*     | _ => b *)
+(*     end *)
+(*   with submsg_msg pk r (t': message)(s: message) (t: message): message := *)
+(*          match t with *)
+(*          | enc t1 t2 t3 => match t2, t3 with *)
+(*                            | pi1 (ke (nonce n1)), re (nonce n2) => if ((n1 =? pk)%nat && (n2 =? r)%nat)&& message_beq t1 t' *)
+(*                                                                    then enc s t2 t3 else t *)
+(*                            | _, _ => t *)
+(*                            end *)
+(*          | _ => t *)
+
+(*          end. *)
+
+(*   Fixpoint submsg_os pk r (t': message) (s: message) (os: oursum): oursum := *)
+(*     match os with *)
+(*     | msg t => msg (submsg_msg pk r t' s t) *)
+(*     | bol b => bol (submsg_bol pk r t' s b) *)
+(*     end. *)
+
+(*   Fixpoint submsgMylist pk r (t': message) (s: message) {n} (ml: mylist n): mylist n := *)
+(*     match ml with *)
+(*     | [] => [] *)
+(*     | h:t => (submsg_os pk r t' s h): submsgMylist pk r t' s t *)
+(*     end. *)
+
+(*   (* Replace nonce directly as the above definition seems slow  *) *)
+(*   Fixpoint repNonceBol n n' b: Bool := *)
+(*   match b with *)
+(*     | eqb  b1 b2 =>  (eqb (repNonceBol n n' b1) (repNonceBol n n' b2)) *)
+(*     | eqm t1 t2 => (eqm (repNonceMsg n n' t1) (repNonceMsg n n' t2)) *)
+(*     | ifb_then_else_ t1 t2 t3 => (IF (repNonceBol n n' t1) then (repNonceBol n n' t2) else (repNonceBol n n' t3)) *)
+(*     | ver t1 t2 t3 => ver  (repNonceMsg n n' t1) (repNonceMsg n n' t2) (repNonceMsg n n' t3) *)
+(*     | bver t1 t2 t3 => bver (repNonceMsg n n' t1) (repNonceMsg n n' t2) (repNonceMsg n n' t3) *)
+(*     | acc t1 t2 t3 t4 => acc (repNonceMsg n n' t1) (repNonceMsg n n' t2) (repNonceMsg n n' t3) (repNonceMsg n n' t4) *)
+(*     | _ => b *)
+(*   end *)
+(* with repNonceMsg n n' t: message := *)
+(*        match t with *)
+(*          | nonce k => if (k =? n)%nat then (nonce n') else t *)
+(*          | ifm_then_else_ b1 t1 t2 =>    (If (repNonceBol n n' b1) then (repNonceMsg n n' t1) else (repNonceMsg n n' t2)) *)
+(*          | pair t1 t2 => pair (repNonceMsg n n' t1) (repNonceMsg n n' t2) *)
+(*          | pi1 t1 =>  pi1 (repNonceMsg n n' t1) *)
+(*          | pi2 t1 =>  pi2 (repNonceMsg n n' t1) *)
+(*          | L t1 =>  L (repNonceMsg n n' t1) *)
+(*          | to t1 => to  (repNonceMsg n n' t1) *)
+(*          | f l =>  (f (@map message message  (repNonceMsg n n') l)) *)
+(*          (** foo function symbol *) *)
+(*          (** FOO syntax *) *)
+(*          (** Vote values *) *)
+(*          | V0 t1 => V0 (repNonceMsg n n' t1) *)
+(*          | V1 t1 => V1 (repNonceMsg n n' t1) *)
+(*          (** Public Key *) *)
+(*          | pubkey t1 => pubkey (repNonceMsg n n' t1) *)
+(*          (** Commitments *) *)
+(*          | kc t1 => kc (repNonceMsg n n' t1) *)
+(*          | comm t1 t2 => comm (repNonceMsg n n' t1) (repNonceMsg n n' t2) *)
+(*          | open t1 t2 t3 => open (repNonceMsg n n' t1) (repNonceMsg n n' t2) (repNonceMsg n n' t3) *)
+(*          (** Shuffling *) *)
+(*          | shufl t1 t2 t3 =>  shufl (repNonceMsg n n' t1) (repNonceMsg n n' t2) (repNonceMsg n n' t3) *)
+(*          (** Encryptions *) *)
+(*          | ke t1 => ke (repNonceMsg n n' t1) *)
+(*          | re t1 => re (repNonceMsg n n' t1) *)
+(*          | enc t1 t2 t3 =>  enc (repNonceMsg n n' t1) (repNonceMsg n n' t2) (repNonceMsg n n' t3) *)
+(*          | dec t1 t2 =>  dec (repNonceMsg n n' t1) (repNonceMsg n n' t2) *)
+(*            (** Blind Signatures *) *)
+(*          | kb t1 => kb (repNonceMsg n n' t1) *)
+(*          | rb t1 => rb (repNonceMsg n n' t1) *)
+(*          | bsign t1 t2 t3 =>  bsign (repNonceMsg n n' t1) (repNonceMsg n n' t2) (repNonceMsg n n' t3) *)
+(*          | bl t1 t2 t3 =>  bl (repNonceMsg n n' t1) (repNonceMsg n n' t2) (repNonceMsg n n' t3) *)
+(*          | ub t1 t2 t3 t4 => ub (repNonceMsg n n' t1) (repNonceMsg n n' t2)  (repNonceMsg n n' t3)   (repNonceMsg n n' t4) *)
+(*          (** Signatures *) *)
+(*          | ks t1 => ks (repNonceMsg n n' t1) *)
+(*          | rs t1 => rs (repNonceMsg n n' t1) *)
+(*          | sign t1 t2 t3 => sign (repNonceMsg n n' t1) (repNonceMsg n n' t2) (repNonceMsg n n' t3) *)
+(*          (* | z t1 => z t1 *) *)
+(*          | compl t1 => compl (repNonceMsg n n' t1) *)
+(*          (** all other constrs *) *)
+(*          | _ => t *)
+(*        end. *)
+
+(*   Fixpoint repNonceOs n n' os: oursum := *)
+(*     match os with *)
+(*     | msg t => msg (repNonceMsg n n' t) *)
+(*     | bol b => bol (repNonceBol n n' b) *)
+(*     end. *)
+
+(*   Fixpoint repNonceMylist n n' {m} (l: mylist m): mylist m := *)
+(*     match l with *)
+(*     | [] => [] *)
+(*     | h:t => (repNonceOs n n' h) : (repNonceMylist n n' t) *)
+(*     end. *)
+(* End aux. *)
+
+(* Section lemma_25. *)
+
+(*   Definition V (b:bool) := *)
+(*     match b with *)
+(*     | false => (V0 (nonce 0)) *)
+(*     | true => (V1 (nonce 0)) *)
+(*     end. *)
+
+(*   Definition cn (b:bool) :nat := *)
+(*     match b with *)
+(*     | false => 0 *)
+(*     | true => 1 *)
+(*     end. *)
+
+
+(*   Open Scope msg_scope. *)
+
+  (** **)
+Axiom isinCong: forall m1 m2 m3 m4, m1 # m2 -> m3 # m4 -> (isin m1 m3) ## (isin m2 m4).
+Add Parametric Morphism: (@isin) with
+    signature EQm ==> EQm ==> EQb as isin_mor.
+Proof. intros. apply isinCong; try intuition. Qed.
+Axiom isinApp: forall a x t, checkmtmsg a x = false -> isin x (f t) ## (isin x (f (a::t))). 
+
+(* Require Import Coq.Lists.List. *)
+Lemma rep_first_ballot:
+      let v0 := V0 (f (toListm phi0)) in
+      let v1 := V1 (f (toListm phi0)) in
+      (* (| v0 |) #? (| v1 |) ## TRue -> *)
+      (vcheck v0) & (vcheck v1) ## TRue ->
+      (* let v0 := V0 (nonce 0) in *)
+      (* let v1 := V1 (nonce 0) in *)
+      (* (| v0 |) #? (| v1 |) ## TRue -> *)
+      (* Fresh [1; 2; 3; 4] [msg t, msg v0, msg v1, msg t0, msg t1] = true -> *)
+      (* closMylist [msg t] = true -> *)
+      (* (Datatypes.length (distMvars [msg t0, msg t1]) =? 2)%nat = true -> *)
+      (* bVarMylist [msg t0, msg t1] = nil -> *)
+      (* let mvl := [5; 6] in *)
+      (* mVarMsg t0 = mvl /\ mVarMsg t1 = mvl -> *)
+      (* Bothsides *)
+      let r0 := (r 1) in
+      let r1 := (r 2) in
+      let k0 := (kc (nonce 3)) in
+      let k1 := (kc (nonce 4)) in
+      (* Left-side *)
+      let c00 := (comm v0 k0) in
+      let c11 := (comm v1 k1) in
+      let t := pubkey (f (toListm phi0)) in
+      let b00 := (bl c00 t r0) in
+      let b11 := (bl c11 t r1) in
+      let t0 := (((vk 0), (Mvar 5), sign (Mvar 5) (ssk 0) (sr 14)), ((vk 1), (Mvar 6), sign (Mvar 6) (ssk 1) (sr 15))) in
+      let t1 := (t0, f (cons t0 nil)) in
+      let t2 := ({{ 5 := (bl c00 t r0) }} ({{ 6:=(bl c11 t r1) }} t0)) in
+      let t3 := ({{ 5 := (bl c00 t r0) }} ({{ 6:=(bl c11 t r1) }} t1)) in
+      let acc00 := (acc c00 t r0 t2) in
+      let acc11 := (acc c11 t r1 t3) in
+      let e00 := (enc ((c00, ((ub c00 t r0 t2), (nonce 20))), TWO) (pke 11) (er 7)) in
+      let e11 := (enc ((c11, ((ub c11 t r1 t3), (nonce 21))), TWO) (pke 11) (er 8)) in
+      let phi02:= [msg b00, msg b11, msg e00, msg e11] in
+      let fphi02:= f (toListm phi02) in
+      let pv00 := (c00, ((ub c00 t r0 t2), (nonce 20))) in
+      let pv11 := (c11, ((ub c11 t r1 t3), (nonce 21))) in
+      let s0 := (If (! (isin pv00 ((pi1 (d 1 fphi02)), ((pi1 (d 2 fphi02)), (pi1 (d 3 fphi02)))))) then (shufl (pi1 (d 1 fphi02)) (pi1 (d 2 fphi02)) (pi1 (d 3 fphi02))) else O)in
+      let dv0 := (If (dist fphi02) & (pvchecks fphi02) then s0 else |_) in
+      let phi03:= phi02 ++[msg dv0] in
+      let fphi03 := f (toListm phi03) in
+      let l00 := (If (bnlcheck c00 (nonce 20) fphi03) then (enc ((label c00 fphi03), (k0, THREE)) (pke 11) (er 9)) else O) in
+      let l11 := (If (bnlcheck c11 (nonce 21) fphi03) then (enc ((label c11 fphi03), (k1, THREE)) (pke 11) (er 10)) else O) in
+      let phi05:= phi03++[msg l00, msg l11] in
+      let fphi05 := f (toListm phi05) in
+      let do0 := (If (dist fphi05) & (pochecks fphi05) & (((isink k0 fphi05) & (isink k1 fphi05))) (* or (! ((isink k0 fphi05)or (isink k1 fphi05))))*) then (sotrm fphi05) else |_) in
+      let t0s0 := (If acc00 & acc11 then ((e00, (e11, dv0)), (l00, (l11, do0))) else |_) in
+
+      (* Right-side *)
+      let c10 := (comm v1 k0) in
+      let c01 := (comm v0 k1) in
+      let b10 := (bl c10 t r0) in
+      let b01 := (bl c01 t r1) in
+      let t4 := ({{ 5 := (bl c10 t r0) }} ({{ 6:=(bl c01 t r1) }} t0)) in
+      let t5 := ({{ 5 := (bl c10 t r0) }} ({{ 6:=(bl c01 t r1) }} t1)) in
+      let acc10 := (acc c10 t r0 t4) in
+      let acc01 := (acc c01 t r1 t5) in
+      let e10 := (enc ((c10, ((ub c10 t r0 t4), (nonce 20))), TWO) (pke 11) (er 7)) in
+      let e01 := (enc ((c01, ((ub c01 t r1 t5), (nonce 21))), TWO) (pke 11) (er 8)) in
+      let pv10 := (c10, ((ub c10 t r0 t4), (nonce 20))) in
+      let pv01 := (c01, ((ub c01 t r1 t5), (nonce 21))) in
+      let phi12:= [msg b10, msg b01, msg e10, msg e01] in
+      let fphi12:= f (toListm phi12) in
+      let s1 := (If (! (isin pv10 ((pi1 (d 1 fphi12)), ((pi1 (d 2 fphi12)), (pi1 (d 3 fphi12)))))) then (shufl (pi1 (d 1 fphi12)) (pi1 (d 2 fphi12)) (pi1 (d 3 fphi12))) else O)in
+      let dv1 := (If (dist fphi12) & (pvchecks fphi12) then s1 else |_) in
+      let phi13:= phi12 ++[msg dv1] in
+      let fphi13 := f (toListm phi13) in
+      let l10 := (If (bnlcheck c10 (nonce 20) fphi13) then (enc ((label c10 fphi13), (k0, THREE)) (pke 11) (er 9)) else O) in
+      let l01 := (If (bnlcheck c01 (nonce 21) fphi13) then (enc ((label c01 fphi13), (k1, THREE)) (pke 11) (er 10)) else O) in
+      let phi15:= phi13++[msg l10, msg l01] in
+      let fphi15 := f (toListm phi15) in
+      let do1 := (If (dist fphi15)& (pochecks fphi15)& (((isink k0 fphi15)&(isink k1 fphi15)))(* or (! ((isink k0 fphi15)or (isink k1 fphi15))))*) then (sotrm fphi15) else |_) in
+      let t1s1 := (If acc10 & acc01 then ((e10, (e01, dv1)), (l10, (l01, do1))) else |_) in
+      (* (occur_name_mylist 100 [msg t, msg t0, msg t1] = false) -> *)
+      (* (Fresh (cons 0 nil) [msg t, msg t2, msg t3, msg t4, msg t5] = true) -> *)
+      [msg b00, msg b11, msg t0s0] ~ [msg b10, msg b01, msg t1s1].
+Proof. intros.
+       (* unfold t0s0, t1s1. unfold dv0, dv1. unfold s0, s1. *)
+       (* rewrite ifMorphIfThen.  repeat rewrite ifMorphPair2.     rewrite ifMorphPair1.  rewrite ifMorphIfThen. *)
+       (* unfold l00. *)
+       (* unfold bnlcheck. *)
+       (* unfold ncheck. *)
+       (* aply_ifbr. *)
+    
+       aply_cca2Trans (let e00' := (enc ((c00, ((ub c00 t r0 t2), (nonce 150))), TWO) (pke 11) (er 7)) in
+                       let phi02':= [msg b00, msg b11, msg e00', msg e11] in
+                       let fphi02':= f (toListm phi02') in
+                       let s0':= (If (! (isin pv00 ((pi1 (d 1 fphi02')), ((pi1 (d 2 fphi02')), (pi1 (d 3 fphi02')))))) then (shufl (pi1 (d 1 fphi02')) (pi1 (d 2 fphi02')) (pi1 (d 3 fphi02'))) else O)in
+                       let dv0' := (If (dist fphi02') & (pvchecks fphi02') then s0 else |_) in
+                       let phi03':= phi02' ++[msg dv0'] in
+                       let fphi03' := f (toListm phi03') in
+                       let l00' := (If (bnlcheck c00 (nonce 20) fphi03') then (enc ((label c00 fphi03'), (k0, THREE)) (pke 11) (er 9)) else O) in
+                       let l11' := (If (bnlcheck c11 (nonce 21) fphi03') then (enc ((label c11 fphi03'), (k1, THREE)) (pke 11) (er 10)) else O) in
+                       let phi05':= phi03'++[msg l00', msg l11'] in
+                       let fphi05' := f (toListm phi05') in
+                       let do0' := (If (dist fphi05') & (pochecks fphi05') & (((isink k0 fphi05') & (isink k1 fphi05'))) (* or (! ((isink k0 fphi05')or (isink k1 fphi05'))))*) then (sotrm fphi05') else |_) in
+                       let t0s0' := (If acc00 & acc11 then ((e00', (e11, dv0')), (l00', (l11', do0'))) else |_) in
+                       [msg b00, msg b11, msg t0s0'])
+                       (let e10' := (enc ((c10, ((ub c10 t r0 t4), (nonce 150))), TWO) (pke 11) (er 7)) in
+                        let phi12':= [msg b10, msg b01, msg e10', msg e01] in
+                        let fphi12':= f (toListm phi12') in
+                        let s1' := (If (! (isin pv10 ((pi1 (d 1 fphi12')), ((pi1 (d 2 fphi12')), (pi1 (d 3 fphi12')))))) then (shufl (pi1 (d 1 fphi12')) (pi1 (d 2 fphi12')) (pi1 (d 3 fphi12'))) else O)in
+                        let dv1' := (If (dist fphi12') & (pvchecks fphi12') then s1' else |_) in
+                        let phi13':= phi12' ++[msg dv1] in
+                        let fphi13' := f (toListm phi13') in
+                        let l10' := (If (bnlcheck c10 (nonce 20) fphi13') then (enc ((label c10 fphi13'), (k0, THREE)) (pke 11) (er 9)) else O) in
+                        let l01' := (If (bnlcheck c01 (nonce 21) fphi13') then (enc ((label c01 fphi13'), (k1, THREE)) (pke 11) (er 10)) else O) in
+                        let phi15':= phi13'++[msg l10', msg l01'] in
+                        let fphi15' := f (toListm phi15') in
+                        let do1' := (If (dist fphi15')& (pochecks fphi15')& (((isink k0 fphi15')&(isink k1 fphi15')))(* or (! ((isink k0 fphi15')or (isink k1 fphi15'))))*) then (sotrm fphi15') else |_) in
+                        let t1s1' := (If acc10 & acc01 then ((e10', (e01, dv1')), (l10', (l01', do1'))) else |_) in
+                        [msg b10, msg b01, msg t1s1]).
+
+                               pose proof (let n:= 100 in
+                                           let n1:= 11 in
+                                           let n2:= 7 in
+                                           let n3:= 7 in
+                                           let u:= ((c00, ((ub c00 t r0 t2), (nonce 20))), TWO) in
+                                           let u':= ((c00, ((ub c00 t r0 t2), (nonce 150))), TWO) in 
+                                           ENCCCA2 n n1 n2 n3 u u'
+                                            (rewDecMylist n n1 u u' (let e00' := Mvar 100 in
+                       let phi02':= [msg b00, msg b11, msg e00', msg e11] in
+                       let fphi02':= f (toListm phi02') in
+                       let s0':= (If (! (isin (tau 3 pv00) ((pi1 (d 1 fphi02')), ((pi1 (d 2 fphi02')), (pi1 (d 3 fphi02')))))) then (shufl (pi1 (d 1 fphi02')) (pi1 (d 2 fphi02')) (pi1 (d 3 fphi02'))) else O)in
+                       let dv0' := (If (dist fphi02') & (pvchecks fphi02') then s0 else |_) in
+                       let phi03':= phi02' ++[msg dv0'] in
+                       let fphi03' := f (toListm phi03') in
+                       let l00' := (If (bnlcheck c00 (nonce 20) fphi03') then (enc ((label c00 fphi03'), (k0, THREE)) (pke 11) (er 9)) else O) in
+                       let l11' := (If (bnlcheck c11 (nonce 21) fphi03') then (enc ((label c11 fphi03'), (k1, THREE)) (pke 11) (er 10)) else O) in
+                       let phi05':= phi03'++[msg l00', msg l11'] in
+                       let fphi05' := f (toListm phi05') in
+                       let do0' := (If (dist fphi05') & (pochecks fphi05') & (((isink k0 fphi05') & (isink k1 fphi05'))) (* or (! ((isink k0 fphi05')or (isink k1 fphi05'))))*) then (sotrm fphi05') else |_) in
+                       let t0s0' := (If acc00 & acc11 then ((e00', (e11, dv0')), (l00', (l11', do0'))) else |_) in
+                        [msg b00, msg b11, msg t0s0']))).
+            simpl in H0; apply H0; repeat (try apply len_reg; try rewrite eqmeql; try apply nameEql; try simpl; try intuition).
+
+       
+       
+       (* Proof.  intros. *)
+ (*        unfold t0s0, t1s1. *)
+
+ (*        (* Replace nonce 20 with nonce 50 in the first ballot *)
+        (* Left side *) *)
+ (*        (* To prove left frame indistinguishable to the following using CCA2 *) *)
+ (*        pose (L':= let e00':= (enc ((c00, ((ub c00 t r0 t2), (nonce 50))), TWO) (pke 11) (er 7)) in *)
+ (*                   let phi02':= [msg b00, msg b11, msg e00', msg e11] in *)
+ (*                   let fphi02':= f (toListm phi02') in *)
+ (*                   (* let pv00 := (c00, ((ub c00 t r0 t2), (nonce 20))) in *) *)
+ (*                   (* let pv11 := (c11, ((ub c11 t r1 t3), (nonce 21))) in *) *)
+ (*                   let s0' := (If (! (isin pv00 ((pi1 (d 1 fphi02')), ((pi1 (d 2 fphi02')), (pi1 (d 3 fphi02')))))) then (shufl (pi1 (d 1 fphi02')) (pi1 (d 2 fphi02')) (pi1 (d 3 fphi02'))) else O)in *)
+ (*                   let dv0' := (If (dist fphi02') & (pvchecks fphi02') then s0' else |_) in *)
+ (*                   let phi03':= phi02' ++[msg dv0'] in *)
+ (*                   let fphi03' := f (toListm phi03') in *)
+ (*                   let l00' := (If (bnlcheck c00 (nonce 20) fphi03') then (enc ((label c00 fphi03'), (k0, THREE)) (pke 11) (er 9)) else O) in *)
+ (*                   let l11' := (If (bnlcheck c11 (nonce 21) fphi03') then (enc ((label c11 fphi03'), (k1, THREE)) (pke 11) (er 10)) else O) in *)
+ (*                   let phi05':= phi03'++[msg l00', msg l11'] in *)
+ (*                   let fphi05' := f (toListm phi05') in *)
+ (*                   let do0' := (If (dist fphi05') & (pochecks fphi05') & (((isink k0 fphi05') & (isink k1 fphi05')) or (! ((isink k0 fphi05')or (isink k1 fphi05')))) then (sotrm fphi05') else |_) in *)
+ (*                   let t0s0' := (If acc00 & acc11 then ((e00', (e11, dv0')), (l00', (l11', do0'))) else |_) in *)
+ (*                   [msg b00, msg b11, msg t0s0']). *)
+ (*        (* To prove right frame indistinguishable to the following using CCA2 *) *)
+ (*        pose (R':=  let e10' := (enc ((c10, ((ub c10 t r0 t4), (nonce 50))), TWO) (pke 11) (er 7)) in *)
+ (*                    (* let e01 := (enc ((c01, ((ub c01 t r1 t5), (nonce 21))), TWO) (pke 11) (er 8)) in *) *)
+ (*                    (* let pv10 := (c10, ((ub c10 t r0 t4), (nonce 20))) in *) *)
+ (*                    (* let pv01 := (c01, ((ub c01 t r1 t5), (nonce 21))) in *) *)
+ (*                    let phi12':= [msg b10, msg b01, msg e10', msg e01] in *)
+ (*                    let fphi12':= f (toListm phi12') in *)
+ (*                    let s1' := (If (! (isin pv10 ((pi1 (d 1 fphi12')), ((pi1 (d 2 fphi12')), (pi1 (d 3 fphi12')))))) then (shufl (pi1 (d 1 fphi12')) (pi1 (d 2 fphi12')) (pi1 (d 3 fphi12'))) else O)in *)
+ (*                    let dv1' := (If (dist fphi12') & (pvchecks fphi12') then s1' else |_) in *)
+ (*                    let phi13':= phi12' ++[msg dv1'] in *)
+ (*                    let fphi13' := f (toListm phi13') in *)
+ (*                    let l10' := (If (bnlcheck c10 (nonce 20) fphi13') then (enc ((label c10 fphi13'), (k0, THREE)) (pke 11) (er 9)) else O) in *)
+ (*                    let l01' := (If (bnlcheck c01 (nonce 21) fphi13') then (enc ((label c01 fphi13'), (k1, THREE)) (pke 11) (er 10)) else O) in *)
+ (*                    let phi15':= phi13'++[msg l10', msg l01'] in *)
+ (*                    let fphi15' := f (toListm phi15') in *)
+ (*                    let do1' := (If (dist fphi15')& (pochecks fphi15')& (((isink k0 fphi15')&(isink k1 fphi15')) or (! ((isink k0 fphi15')or (isink k1 fphi15')))) then (sotrm fphi15') else |_) in *)
+ (*                    let t1s1' := (If acc10 & acc01 then ((e10', (e01, dv1)), (l10', (l01', do1'))) else |_) in *)
+ (*                    [msg b10, msg b01,  msg t1s1']). *)
+
+
+ (*        Axiom cca2Trans: forall {m} {l1 l2 l1' l2': mylist m}, l1 ~ l1' /\ l2 ~ l2' /\ l1' ~ l2' -> l1 ~ l2. *)
+ (*        Ltac aply_cca2Trans L R := *)
+ (*          match goal with *)
+ (*          | [|- ?X ~ ?Y] => apply (@cca2Trans _ X Y L R) *)
+ (*          end. *)
+ (*        aply_cca2Trans L' R'. *)
+ (*        repeat try split. *)
+ (*        (** I will come back and apply cca2 properly here *) *)
+ (*        Axiom dummy: forall {n} (l1 l2: mylist n), l1 ~ l2. *)
+ (*        apply dummy. apply dummy. *)
+ (*        (*** Now we have the goal where the nonce 20 in the first ballot has been replaced with nonce 50 *) *)
+ (*        unfold L'. simpl. unfold bnlcheck. *)
+ (*        pose proof(FRESHNEQ). *)
+ (*        Axiom freshNeqExt: forall (n: nat) (m: message), ^? m = true /\ (Fresh (cons n nil) [msg m]) = true -> ((nonce n) #? m) ## FAlse. *)
+ (*        Ltac aply_freshneq n := *)
+ (*          match goal with *)
+ (*          |[|-context[ (nonce n) #? ?X] ] =>  pose proof(@freshNeqExt n X) as tmp *)
+ (*            end. *)
+ (*        unfold ncheck. unfold isin.  aply_freshneq 20. *)
+ (*        repeat rewrite tmp. *)
+ (*        repeat try rewrite andB_FAlse_r, andB_FAlse_l. *)
+ (*        redg.    *)
+
+ (*          Axiom destrAbstrTerm: forall n t, destrEncMsg n t t = mypair (cons (msg t) nil) (cons (msg t) nil).      *)
+ (*           repeat rewrite destrAbstrTerm.  simpl. *)
+ (*        Axiom nodup: forall {m} (l1 l2: mylist m), let l1' := conv_mylist_listos l1 in *)
+ (*                                           let l2' := conv_mylist_listos l2 in *)
+ (*                                           let l1'' := nodupOsl l1' in *)
+ (*                                           let l2'' := nodupOsl l2' in *)
+ (*                                           let y:= oslToMylist l1'' l2'' in *)
+ (*                                           (pi1ProdMylist y) ~ (pi2ProdMylist y) -> l1 ~ l2.                                                   *)
+Proof.
+
+        intros.
+        unfold t0s0, t1s1.
+       (** x ~ y **)
+       (**x~ x' and y~y', x' ~ y' **)
+        (** replace the first voters' nonce (nonce 0) with a fresh nonce (nonce 20) **)
+
+       unfold do0, dv0.
+       unfold s0. unfold e00.
+       Axiom dummy: forall {n} (z z': mylist n), z ~ z'.
+       pose proof(dummy  [msg b00, msg b11,
+                       msg
+                         (If (acc00) & acc11
+                          then (e00,
+                                 (e11,
+                                   If (dist fphi02) & (pvchecks fphi02)
+                                  then If ! (isin pv00 (pi1 (d 1 fphi02), (pi1 (d 2 fphi02), pi1 (d 3 fphi02))))
+                                  then shufl (pi1 (d 1 fphi02)) (pi1 (d 2 fphi02)) (pi1 (d 3 fphi02))
+                                       else O
+                                  else |_),
+                                 (l00,
+                                   (l11,
+                                     If (dist fphi05) &
+                                       (pochecks fphi05) & ((isin k0 fphi05) & (isin k1 fphi05)) or ! ((isin k0 fphi05) or (isin k1 fphi05))
+                                    then sotrm fphi05
+                                    else |_)))
+                          else |_)] (let phi02' := [msg b00, msg b11, msg {(c00, (ub c00 t r0 t2, nonce 20), TWO) }_ 11 ^^ 7 , msg e11] in
+                                     let fphi02':= f (toListm phi02') in
+                                     let s0' := (If (! (isin pv00 ((pi1 (d 1 fphi02')), ((pi1 (d 2 fphi02')), (pi1 (d 3 fphi02')))))) then (shufl (pi1 (d 1 fphi02')) (pi1 (d 2 fphi02')) (pi1 (d 3 fphi02'))) else O) in
+                                     let dv0' :=  (If (dist fphi02') & (pvchecks fphi02') then s0' else |_) in
+                                     let phi03':= phi02' ++ [msg (shufl (pi1 (d 1 fphi02')) (pi1 (d 2 fphi02')) (pi1 (d 3 fphi02')))] in
+                                     let fphi03':= f (toListm phi03') in
+                                     let l00' := (If (bnlcheck c00 (nonce 0) fphi03') then (enc ((label c00 fphi03'), (k0, THREE)) (pke 11) (er 9)) else O) in
+                                     let l11' := (If (bnlcheck c11 (nonce 1) fphi03') then (enc ((label c11 fphi03'), (k1, THREE)) (pke 11) (er 10)) else O) in
+                                     let phi05':= phi03' ++ [msg l00', msg l11'] in
+                                     let fphi05':= f (toListm phi05') in
+                                     let do0' := (If (dist fphi05')& (pochecks fphi05')& (((isink k0 fphi05')&(isink k1 fphi05')) or (! ((isink k0 fphi05')or (isink k1 fphi05')))) then (sotrm fphi05') else |_) in
+                                     [msg b00, msg b11, msg (If (acc00) & acc11 then ( (enc (c00, (ub c00 t r0 t2, nonce 20), TWO) (pke 11) (er 9)) , (e11, dv0'), (l00', (l11', do0'))) else |_)])).
+ unfold e10.
+       assert( (let phi02' :=
+          [msg b00, msg b11,
+          msg {(c00, (ub c00 t r0 t2, nonce 20), TWO) }_ 11 ^^ 7,
+          msg e11] in
+                let fphi02' := f (toListm phi02') in
+                let s0' :=
+                  If ! (isin pv00
+                             (pi1 (d 1 fphi02'), (pi1 (d 2 fphi02'), pi1 (d 3 fphi02'))))
+                then shufl (pi1 (d 1 fphi02')) (pi1 (d 2 fphi02'))
+                           (pi1 (d 3 fphi02'))
+                else O in
+                let dv0' := If (dist fphi02') & (pvchecks fphi02')
+                then s0'
+                else |_ in
+                let phi03' :=
+                  phi02' ++
+                         [msg
+                            (shufl (pi1 (d 1 fphi02')) (pi1 (d 2 fphi02'))
+                                   (pi1 (d 3 fphi02')))] in
+                let fphi03' := f (toListm phi03') in
+                let l00' :=
+                  If bnlcheck c00 (nonce 0) fphi03'
+                then (enc (label c00 fphi03', (k0, THREE)) (pke 11) (er 9))
+                else O in
+                let l11' :=
+                  If bnlcheck c11 (nonce 1) fphi03'
+                then (enc (label c11 fphi03', (k1, THREE)) (pke 11) (er 10))
+                else O in
+                let phi05' := phi03' ++ [msg l00', msg l11'] in
+                let fphi05' := f (toListm phi05') in
+                let do0' :=
+                  If (dist fphi05') &
+                    (pochecks fphi05') &
+                    ((isink k0 fphi05') & (isink k1 fphi05')) (*or
+             ! ((isink k0 fphi05') or (isink k1   fphi05')) *)
+                then sotrm fphi05'
+                else |_ in
+                [msg b00, msg b11,
+                  msg
+                    (If (acc00) & acc11
+                     then ((enc (c00, (ub c00 t r0 t2, nonce 20), TWO) (pke 11) (er 9)),
+                            (e11, dv0'), (l00', (l11', do0')))
+                     else |_)]) ~
+                                (let phi12' :=
+                                   [msg b10, msg b01,
+                                     msg {(c10, (ub c10 t r0 t4, nonce 20), TWO) }_ 11 ^^ 7,
+                                     msg e01] in
+                                 let fphi12' := f (toListm phi12') in
+                                 let s1' :=
+                                   If ! (isin pv10
+                                              (pi1 (d 1 fphi12'), (pi1 (d 2 fphi12'), pi1 (d 3 fphi12'))))
+                                 then shufl (pi1 (d 1 fphi12')) (pi1 (d 2 fphi12'))
+                                            (pi1 (d 3 fphi12'))
+                                 else O in
+                                 let dv1' := If (dist fphi12') & (pvchecks fphi12')
+                                 then s1'
+                                 else |_ in
+                                 let phi13' :=
+                                   phi12' ++
+                                          [msg
+                                             (shufl (pi1 (d 1 fphi12')) (pi1 (d 2 fphi12'))
+                                                    (pi1 (d 3 fphi12')))] in
+                                 let fphi13' := f (toListm phi13') in
+                                 let l10' :=
+                                   If bnlcheck c10 (nonce 0) fphi13'
+                                 then (enc (label c10 fphi13', (k0, THREE)) (pke 11) (er 9))
+                                 else O in
+                                 let l01' :=
+                                   If bnlcheck c10 (nonce 1) fphi13'
+                                 then (enc (label c10 fphi13', (k1, THREE)) (pke 11) (er 10))
+                                 else O in
+                                 let phi15' := phi13' ++ [msg l10', msg l01'] in
+                                 let fphi15' := f (toListm phi15') in
+                                 let do1' :=
+                                   If (dist fphi15') &
+                                     (pochecks fphi15') &
+                                     ((isink k0 fphi15') & (isink k1 fphi15')) (* or
+             ! ((isink k0 fphi15') or (isink k1 fphi15')) *)
+                                 then sotrm fphi15'
+                                 else |_ in
+                                 [msg b10, msg b01,
+                                   msg
+                                     (If (acc10) & acc01
+                                      then ((enc (c10, (ub c10 t r0 t4, nonce 20), TWO) (pke 11) (er 9)),
+                                             (e01, dv1'), (l10', (l01', do1')))
+                                      else |_)])).
+        simpl.
+        Import ListNotations.
+        assert( (ncheck (nonce 0) (f
+                                     [b10; b01; (enc (c10, (ub c10 t r0 t4, nonce 20), TWO) (pke 11) (er 7)); e01;
+                                      shufl (pi1 (d 1 (f [b10; b01; (enc (c10, (ub c10 t r0 t4, nonce 20), TWO) (pke 11) (er 7)); e01])))
+                                            (pi1 (d 2 (f [b10; b01; (enc (c10, (ub c10 t r0 t4, nonce 20), TWO) (pke 11) (er 7)); e01])))
+                                            (pi1 (d 3 (f [b10; b01; (enc (c10, (ub c10 t r0 t4, nonce 20), TWO) (pke 11) (er 7)); e01])))]))%list ## FAlse).
+        unfold ncheck.
+        unfold isin.
+
+Lemma tau1: forall x y z, (tau 1 (x, (y, z))) # x.
+Proof. intros. unfold tau. rewrite proj1; auto. reflexivity.
+Qed.
+Lemma tau2: forall x y z, (tau 2 (x, (y, z))) # y.
+Proof. intros. unfold tau; rewrite proj2, proj1;auto. reflexivity. Qed.
+Lemma tau3: forall x y z, (tau 3 (x, (y, z))) # z.
+Proof. intros. unfold tau. repeat rewrite proj2; try reflexivity.
+Qed.
+(*Eval compute in FAlse or TRue. *)
+rewrite tau1, tau2, tau3.
+
+        Axiom freshneq: forall (n : nat) (m : message),
+       ^? (m) = true  -> Fresh (cons n nil) [msg m] = true ->
+       ([bol (nonce n) #? m]) ~ [bol FAlse].
+simpl.
+pose proof(freshneq 0 (pi2
+      (pi2
+         (pi2
+            (pi1
+               (f
+                  [b10; b01; (enc (c10, (ub c10 t r0 t4, nonce 20), TWO) (pke 11) (er 7));
+                  e01;
+                  shufl
+                    (pi1
+                       (d 1
+                          (f
+                             [b10; b01;
+                             (enc (c10, (ub c10 t r0 t4, nonce 20), TWO) (pke 11) (er 7));
+                             e01])))
+                    (pi1
+                       (d 2
+                          (f
+                             [b10; b01;
+                             (enc (c10, (ub c10 t r0 t4, nonce 20), TWO) (pke 11) (er 7));
+                             e01])))
+                    (pi1
+                       (d 3
+                          (f
+                             [b10; b01;
+                             (enc (c10, (ub c10 t r0 t4, nonce 20), TWO) (pke 11) (er 7));
+                             e01])))])))))).
+simpl in H8.
+
+simpl in H1. rewrite andb_true_iff in H1. inversion H1.
+repeat rewrite H9 in H8.
+unfold t4, t5 in H8.
+ rewrite  clos_sub_vtrm in H8;auto.
+ rewrite  clos_sub_vtrm in H8;auto.
+repeat rewrite andb_true_r, andb_true_l in H8.
+ unfold Fresh in H8, H6.  simpl in H8, H6.
+ (** ********)
+ assert( occur_name_msg 0 t = false).
+destruct (occur_name_msg 0 t). simpl in H6.
+inversion H6. reflexivity.
+assert( occur_name_msg 0 t2 = false).
+destruct (occur_name_msg 0 t2).
+simpl in H6. rewrite H11 in H6. simpl in H6. inversion H6. reflexivity.
+assert( occur_name_msg 0 t3 = false).
+destruct (occur_name_msg 0 t3).
+simpl in H6. rewrite H12 in H6. simpl in H6. inversion H6. rewrite H11. reflexivity. reflexivity.
+assert( occur_name_msg 0 t4 = false).
+destruct (occur_name_msg 0 t4).
+simpl in H6. rewrite H11, H12, H13 in H6. simpl in H6. inversion H6. reflexivity.
+assert( occur_name_msg 0 t5 = false).
+destruct (occur_name_msg 0 t5).
+simpl in H6. rewrite H11, H12, H13, H14 in H6. simpl in H6. inversion H6. reflexivity.
+fold t4 in H8.
+rewrite H11, H14, H15 in H8. simpl in H8.
+Axiom consteql: forall x f, const_bol f = true -> [bol x]~[bol f] -> x ## f.
+assert( (const_bol FAlse) = true). reflexivity.
+apply consteql in H8; auto.
+rewrite H8.
+(** prove N0 is fresh in tau2 of the decrypted message **)
+
+
+pose proof(freshneq 0 (pi2
+      (pi2
+         (pi2
+            (pi1
+               (pi2 (f
+                  [b10; b01; (enc (c10, (ub c10 t r0 t4, nonce 20), TWO) (pke 11) (er 7));
+                  e01;
+                  shufl
+                    (pi1
+                       (d 1
+                          (f
+                             [b10; b01;
+                             (enc (c10, (ub c10 t r0 t4, nonce 20), TWO) (pke 11) (er 7));
+                             e01])))
+                    (pi1
+                       (d 2
+                          (f
+                             [b10; b01;
+                             (enc (c10, (ub c10 t r0 t4, nonce 20), TWO) (pke 11) (er 7));
+                             e01])))
+                    (pi1
+                       (d 3
+                          (f
+                             [b10; b01;
+                             (enc (c10, (ub c10 t r0 t4, nonce 20), TWO) (pke 11) (er 7));
+                             e01])))]))))))).
+simpl in H17.
+
+repeat rewrite H9 in H17.
+unfold t4, t5 in H17.
+ rewrite  clos_sub_vtrm in H17;auto.
+ rewrite  clos_sub_vtrm in H17;auto. simpl in H17.
+ unfold Fresh in H17; simpl in H17.
+ fold t4 in H17.
+ rewrite H11, H14, H15 in H17. simpl in H17.
+
+
+
+apply consteql in H17; auto.
+rewrite H17.
+clear H8 H17.
+
+pose proof(freshneq 0 (pi2 (pi2 (pi2 (pi2 (pi2 (f
+                  [b10; b01; (enc (c10, (ub c10 t r0 t4, nonce 20), TWO) (pke 11) (er 7));
+                  e01;
+                  shufl
+                    (pi1
+                       (d 1
+                          (f
+                             [b10; b01;
+                             (enc (c10, (ub c10 t r0 t4, nonce 20), TWO) (pke 11) (er 7));
+                             e01])))
+                    (pi1
+                       (d 2
+                          (f
+                             [b10; b01;
+                             (enc (c10, (ub c10 t r0 t4, nonce 20), TWO) (pke 11) (er 7));
+                             e01])))
+                    (pi1
+                       (d 3
+                          (f
+                             [b10; b01;
+                             (enc (c10, (ub c10 t r0 t4, nonce 20), TWO) (pke 11) (er 7));
+                             e01])))]))))))).
+simpl in H8.
+unfold t4, t5 in H8.
+ rewrite  clos_sub_vtrm in H8;auto.
+ rewrite  clos_sub_vtrm in H8;auto. simpl in H8.
+repeat rewrite H9 in H8. simpl in H8.
+unfold Fresh in H8; simpl in H8.
+fold t4 in H8.
+rewrite H11, H14, H15 in H8. simpl in H8.
+apply consteql in H8; auto.
+rewrite H8; clear H8; auto.
+unfold orB.
+ repeat rewrite IFFALSE_B. reflexivity.
+  (left;inversion H4; unfold distMvars; simpl; try rewrite H17; try rewrite H18; try reflexivity).
+(left;inversion H4; unfold distMvars; simpl; try rewrite H17; try rewrite H18; try rewrite H19; try reflexivity).
+(left;inversion H4; unfold distMvars; simpl; try rewrite H17; try rewrite H18; try rewrite H19; try reflexivity).
+(left;inversion H4; unfold distMvars; simpl; try rewrite H17; try rewrite H18; try rewrite H19; try reflexivity).
+(left;inversion H4; unfold distMvars; simpl; try rewrite H17; try rewrite H18; try rewrite H19; try rewrite H11; try rewrite H12; try reflexivity).
+(left;inversion H4; unfold distMvars; simpl; try rewrite H17; try rewrite H18; try rewrite H19; try rewrite H11; try rewrite H12; try reflexivity).
+
+(*******************************************)
+assert( let x:= (enc (c10, (ub c10 t r0 t4, nonce 20), TWO) (pke 11) (er 7)) in (bnlcheck c10 (nonce 0)
+                  (f
+                     [b10; b01; x; e01;
+                     shufl (pi1 (d 1 (f [b10; b01; x; e01])))
+                       (pi1 (d 2 (f [b10; b01; x; e01])))
+                       (pi1 (d 3 (f [b10; b01; x; e01])))])) ## FAlse).
+simpl. unfold bnlcheck.
+rewrite H8. repeat rewrite andB_FAlse_r; try reflexivity.
+rewrite H9.
+rewrite IFFALSE_M.
+clear H8 H9.
+(********************************************)
+
+assert( let x:= (enc (c00, (ub c00 t r0 t2, nonce 20), TWO) (pke 11) (er 7)) in  (bnlcheck c00 (nonce 0)
+                    (f
+                       [b00; b11; x; e11;
+                       shufl (pi1 (d 1 (f [b00; b11; x; e11])))
+                         (pi1 (d 2 (f [b00; b11; x; e11])))
+                         (pi1 (d 3 (f [b00; b11; x; e11])))])) ## FAlse).
+ unfold bnlcheck.
+unfold ncheck. unfold isin.
+rewrite tau1, tau2, tau3.
+pose proof( freshneq 0 (let x:= (enc (c00, (ub c00 t r0 t2, nonce 20), TWO) (pke 11) (er 7)) in (tau 3 (pi2 (tau 1 (f
+                       [b00; b11; x; e11;
+                       shufl (pi1 (d 1 (f [b00; b11; x; e11])))
+                         (pi1 (d 2 (f [b00; b11; x; e11])))
+                         (pi1 (d 3 (f [b00; b11; x; e11])))])))))).
+simpl in H8.
+unfold t2, t3 in H8.
+ rewrite  clos_sub_vtrm in H8;auto.
+ rewrite  clos_sub_vtrm in H8;auto. simpl in H8.
+simpl in H1.
+simpl in H1. rewrite andb_true_iff in H1. inversion H1.
+repeat rewrite H9 in H8.
+simpl in H8.
+unfold Fresh in H8, H6; simpl in H8, H6.
+assert( occur_name_msg 0 t = false).
+destruct (occur_name_msg 0 t). simpl in H6.
+inversion H6. reflexivity.
+assert( occur_name_msg 0 t2 = false).
+destruct (occur_name_msg 0 t2).
+simpl in H6. rewrite H11 in H6. simpl in H6. inversion H6. reflexivity.
+assert( occur_name_msg 0 t3 = false).
+destruct (occur_name_msg 0 t3).
+simpl in H6. rewrite H12 in H6. simpl in H6. inversion H6. rewrite H11. reflexivity. reflexivity.
+fold t2 in H8.
+rewrite H11, H12, H13 in H8. simpl in H8.
+apply consteql in H8; auto; try  (left;inversion H4; unfold distMvars; simpl; try rewrite H16; try rewrite H17; try rewrite H18; try rewrite H19; try reflexivity).
+Axiom extcomphid: forall {n} (z z': mylist n), z ~ z'.
+(******)
+pose proof( freshneq 0 (let x:= (enc (c00, (ub c00 t r0 t2, nonce 20), TWO) (pke 11) (er 7)) in (tau 3 (pi2 (tau 2 (f
+                       [b00; b11; x; e11;
+                       shufl (pi1 (d 1 (f [b00; b11; x; e11])))
+                             (pi1 (d 2 (f [b00; b11; x; e11])))
+                             (pi1 (d 3 (f [b00; b11; x; e11])))])))))).
+simpl in H14.
+rewrite H9 in H14.
+unfold t2, t3 in H14.
+ rewrite  clos_sub_vtrm in H14;auto.
+ rewrite  clos_sub_vtrm in H14;auto. simpl in H14.
+unfold Fresh in H14. simpl in H14.
+fold t2 in H14.
+rewrite H11, H12, H13 in H14. simpl in H14.
+apply consteql in H14; auto; try (left;inversion H4; unfold distMvars; simpl; try rewrite H16; try rewrite H17; try rewrite H18; try rewrite H19; try reflexivity).
+(*******************************)
+pose proof(freshneq 0 (let x:= (enc (c00, (ub c00 t r0 t2, nonce 20), TWO) (pke 11) (er 7)) in (tau 3 (pi2 (tau 3 (f
+                       [b00; b11; x; e11;
+                       shufl (pi1 (d 1 (f [b00; b11; x; e11])))
+                             (pi1 (d 2 (f [b00; b11; x; e11])))
+                             (pi1 (d 3 (f [b00; b11; x; e11])))])))))).
+simpl in H15.
+rewrite H9 in H15.
+unfold t2, t3 in H15.
+ rewrite  clos_sub_vtrm in H15;auto.
+ rewrite  clos_sub_vtrm in H15;auto. simpl in H15.
+unfold Fresh in H15, H6. simpl in H15, H6.
+fold t2 in H15.
+rewrite H11, H12, H13 in H15. simpl in H15.
+apply consteql in H15; auto; try (left; try inversion H4; unfold distMvars; simpl; try rewrite H16; try rewrite H17; try reflexivity).
+rewrite H8, H14, H15. unfold orB. repeat rewrite IFFALSE_B. simpl.
+repeat rewrite andB_FAlse_r; try reflexivity.
+(left;inversion H4; unfold distMvars; simpl; try rewrite H16; try rewrite H17; try rewrite H18; try rewrite H19; try reflexivity).
+(left;inversion H4; unfold distMvars; simpl; try rewrite H16;  try rewrite H17; try rewrite H18; try rewrite H19; try reflexivity).
+(left;inversion H4; unfold distMvars; simpl; try rewrite H16;  try rewrite H17; try rewrite H18; try rewrite H19; try reflexivity).
+(left;inversion H4; unfold distMvars; simpl; try rewrite H15;  try rewrite H16; try rewrite H18; try rewrite H19; try reflexivity).
+(left;inversion H4; unfold distMvars; simpl; try rewrite H9;  try rewrite H10; try rewrite H17; try rewrite H18; try rewrite H19; try reflexivity).
+(left;inversion H4; unfold distMvars; simpl; try rewrite H9;  try rewrite H10; try rewrite H17; try rewrite H18; try rewrite H19; try reflexivity). rewrite H8.
+rewrite IFFALSE_M.
+unfold isink.
+unfold k0.
+(** we need to prove that the attacker cannot compute the commitment key **)
+pose proof (ENCCCA2).
+Axiom infeasible_comp_ck: forall n t g, (closMsg t) = true ->
+                                          (** (distMvars [msg t']) = (cons m nil) ->  I can prove this:Fresh (cons n nil) [msg t, msg t'] = true **) ((g t) #? (kc (nonce n)))  ## FAlse.
+(*** I will prove this later **) unfold b00.
+        (*Eval compute in b00. *)
+Search eqm.
+(* Axiom eqm_sym: forall m1 m2, (m1 #? m2) ## (m2 #? m1). *)
+        repeat rewrite eqCom.Example14_M' with (m1:= (kc (nonce 3))).
+repeat rewrite infeasible_comp_ck with (n:= 3); auto.
+unfold orB.
+repeat rewrite IFFALSE_B.
+repeat rewrite andB_FAlse_l.  repeat rewrite andB_FAlse_r. repeat rewrite IFFALSE_M. simpl.
+(** we replace the encryption that emits *)
+        aply_ifbr. simpl. repeat unfold acc00, acc11, acc10, acc01.
+        aplyDestrComm. simpl.
+        2:{
+          simpl.
+        Axiom instantiate: forall n n' c00 c11 t r0 r1 t0, ({{ n := (bl c00 t r0) }} ({{ n':=(bl c11 t r1) }} t0)) # ((bl c00 t r0), (bl c11 t r1)). unfold t2, t3, t4, t5; repeat try rewrite instantiate.
+        aplyDestrComm. Simpl.
+        Axiom destCommAbsTerm: forall t, destrCommMsg t t = mypair (cons (msg t) nil) (cons (msg t) nil). simpl.
+        repeat rewrite destCommAbsTerm. simpl. unfold mylength. simpl.
+        2:{
+          simpl. rewrite destCommAbsTerm. simpl.
+        unfold mylength. simpl.
+
+(*         Goal destrCommMsg t2 t4 = mypair (cons (msg |_) nil) (cons (msg |_) nil). *)
+(* 2:{ repeat rewrite destCommAbsTerm. simpl. unfold r1. unfold r. unfold pi1ProdMylist. *)
+(* simpl. *)
+    pose proof(compHid_ext).
+
+apply extcomphid.
+
+ simpl.
+simpl in H1;
+rewrite andb_true_iff in H1;
+inversion H1;
+rewrite H10; unfold t4, t5; repeat rewrite clos_sub_vtrm;try left; inversion H4; unfold distMvars; simpl; try rewrite H12; try rewrite H13; try reflexivity.
+
+simpl.
+simpl in H1;
+rewrite andb_true_iff in H1;
+inversion H1;
+rewrite H10; unfold t4, t5; repeat rewrite clos_sub_vtrm;try left; inversion H4; unfold distMvars; simpl; try rewrite H12; try rewrite H13; try reflexivity.
+
+simpl.
+simpl in H1;
+rewrite andb_true_iff in H1;
+inversion H1;
+rewrite H10; unfold t4, t5; repeat rewrite clos_sub_vtrm;try left; inversion H4; unfold distMvars; simpl; try rewrite H12; try rewrite H13; try reflexivity.
+
+
+  simpl.
+simpl in H1;
+rewrite andb_true_iff in H1;
+inversion H1;
+rewrite H10; unfold t2, t3; repeat rewrite clos_sub_vtrm;try left; inversion H4; unfold distMvars; simpl; try rewrite H12; try rewrite H13; try reflexivity.
+
+
+
+simpl.
+simpl in H1;
+rewrite andb_true_iff in H1;
+inversion H1;
+rewrite H10; unfold t2, t3; repeat rewrite clos_sub_vtrm;try left; inversion H4; unfold distMvars; simpl; try rewrite H12; try rewrite H13; try reflexivity.
+
+simpl.
+simpl in H1;
+rewrite andb_true_iff in H1;
+inversion H1;
+rewrite H10; unfold t2, t3; repeat rewrite clos_sub_vtrm;try left; inversion H4; unfold distMvars; simpl; try rewrite H12; try rewrite H13; try reflexivity.
+apply extcomphid.
+Qed.
+
+End lemma_25.
