src/voteprivacy/lemma_25.v
@@ -1,7 +1,7 @@
 (************************************************************************)
 (* Copyright (c) 2017-2018, Ajay Kumar Eeralla <ae266@mail.missouri.edu>*)
 (************************************************************************)
-Require Export contexts.
+Require Export newCca2Compliant.
 Import ListNotations.
 
 (** Simplified CCA2 axiom **)
@@ -14,12 +14,13 @@ Import ListNotations.
 
 (* This should be provable from freshNeq *)
 Axiom bnlcheckFailForNonce: forall n t1 t2, closMsg t2 = true ->
-                                            Fresh (cons n nil) [msg t2] = true -> (bnlcheck t1 (nonce n) t2) ## FAlse.
+                                            Fresh (cons n nil) [msg t2] = true ->
+                                            (bnlcheck t1 (nonce n) t2) ## FAlse.
 
 Ltac rewBnlchkFailNonce c n1 :=
   repeat match goal with
-         |[|- context[bnlcheck c (nonce n1) _] ]=> rewrite bnlcheckFailForNonce with (n:= n1) (t1:= c);
-                                                   try unfold Fresh; simpl; intuition
+         | [|- context[bnlcheck c (nonce n1) _] ] => rewrite bnlcheckFailForNonce with (n:= n1) (t1:= c);
+                                                      try unfold Fresh; simpl; intuition
          end.
 
 Fixpoint and (l: list bool): bool :=
@@ -44,14 +45,34 @@ Ltac rewAndBFalse :=
          end; redg.
 
 
-Axiom ifMorphMsg: forall f b t1 t2, f (If b then t1 else t2) # (If b then (f t1) else (f t2)). 
+Axiom ifMorphMsg: forall f b t1 t2, f (If b then t1 else t2) # (If b then (f t1) else (f t2)).
 Axiom ifMorphBol: forall f b t1 t2, f (If b then t1 else t2)  ## (IF b then (f t1) else (f t2)).
-Import Cxt.
+
+Import CxtCompHid.
+
 Axiom funcAppRestr: forall p1 p2 {m} (l1 l2: mylist m) {f: message -> message -> oslist},
     (IsContextOslist f) ->
     l1 ~ l2 ->
     let osl1:= (f (ostomsg (getelt_at_pos p1 l1)) (ostomsg (getelt_at_pos p2 l1))) in
     let osl2:= (f (ostomsg (getelt_at_pos p1 l2)) (ostomsg (getelt_at_pos p2 l2))) in
+    let y := oslToMylist osl1 osl2 in
+    ((mylength y) =? 0 = false)%nat -> (pi1ProdMylist y) ~ (pi2ProdMylist y).
+
+Import cca2Compliant.
+
+Fixpoint occur_name_oslist (x:nat) (l: oslist) :bool :=
+  match l with
+    | [ ] => false
+    | h :: ml1 =>  (occurOs x h) || (occur_name_oslist x ml1)
+  end.
+
+Axiom cca2CxtAxiom: forall n n1 n2 u u' {f: message -> oslist},
+    (|u| #? |u'|) ## TRue ->
+    (IsContextCCA2Oslist n f) ->
+    occur_name_oslist n1 (f O) = false ->
+    occur_name_oslist n2 (f O) = false ->
+    let osl1:= (f {u}_n^^n1) in
+    let osl2:= (f {u'}_n^^n2) in
     let y := oslToMylist osl1 osl2 in
     ((mylength y) =? 0 = false)%nat -> (pi1ProdMylist y) ~ (pi2ProdMylist y).
 
@@ -66,11 +87,22 @@ Axiom funcAppRestrCompHid: forall n1 n2 v0 v1 {f: message -> message -> oslist},
     let c01:= (comm v0 (kc (nonce n2))) in
     [msg c00, msg c11 ] ~ [msg c10, msg c01] ->
     let osl1:= (f c00 c11) in
-    let osl2:= (f c10 c01) in 
+    let osl2:= (f c10 c01) in
     let y := oslToMylist osl1 osl2 in
     ((mylength y) =? 0 = false)%nat -> (pi1ProdMylist y) ~ (pi2ProdMylist y).
 
+Axiom simplifyGoal: forall {n m o} (l: mylist n) (l1 l2: mylist m) {g: mylist m -> mylist o}, (l ++ l1) ~ (l ++ l2) -> (l ++ (g l1)) ~ (l ++ (g l2)).
 
+Axiom funcApp_t0_t1 : forall n m p1 p2 t0 t1 {n1} (l1 l2: mylist n1), l1 ~ l2 ->
+               let s0 := ostomsg (getelt_at_pos p1 l1) in
+               let s1 := ostomsg (getelt_at_pos p2 l1) in
+               let s0' := ostomsg (getelt_at_pos p1 l2) in
+               let s1' := ostomsg (getelt_at_pos p2 l2) in
+               (l1 ++ [msg ({{ n := s0 }} ({{ m := s1 }} t0)), msg ({{ n := s0 }} ({{ m := s1 }} t1))]) ~  (l2 ++ [msg ({{ n := s0' }} ({{ m := s1' }} t0)), msg ({{ n := s0' }} ({{ m := s1' }} t1))]).
+
+Add Parametric Morphism: (@ isin) with
+           signature EQm ==> EQm ==> EQb as isin_mor.
+       Proof. intros; aply_cong; try auto. Qed.
 
 Lemma rep_first_ballot:
       let v0 := V0 (f (toListm phi0)) in
@@ -133,11 +165,11 @@ Lemma rep_first_ballot:
       let fphi12:= f (toListm phi12) in
       let s1 := (If (! (isin pv10 ((pi1 (d 1 fphi12)), ((pi1 (d 2 fphi12)), (pi1 (d 3 fphi12)))))) then (shufl (pi1 (d 1 fphi12)) (pi1 (d 2 fphi12)) (pi1 (d 3 fphi12))) else O)in
       let dv1 := (If (dist fphi12) & (pvchecks fphi12) then s1 else |_) in
-      let phi13:= phi12 ++[msg dv1] in
+      let phi13:= phi12 ++ [msg dv1] in
       let fphi13 := f (toListm phi13) in
       let l10 := (If (bnlcheck c10 (nonce 20) fphi13) then (enc ((label c10 fphi13), (k0, THREE)) (pke 11) (er 9)) else O) in
       let l01 := (If (bnlcheck c01 (nonce 21) fphi13) then (enc ((label c01 fphi13), (k1, THREE)) (pke 11) (er 10)) else O) in
-      let phi15:= phi13++[msg l10, msg l01] in
+      let phi15:= phi13 ++[msg l10, msg l01] in
       let fphi15 := f (toListm phi15) in
       let do1 := (If (dist fphi15)& (pochecks fphi15)& (((isink k0 fphi15)&(isink k1 fphi15))) (*or (! ((isink k0 fphi15)or (isink k1 fphi15))))*) then (sotrm fphi15) else |_) in
       let t1s1 := (If acc10 & acc01 then ((e10, (e01, dv1)), (l10, (l01, do1))) else |_) in
@@ -145,12 +177,11 @@ Lemma rep_first_ballot:
 (*********Proof starts from here********)
 
 Proof. intros.
-            
-      
        aply_cca2Trans (let e00' := (enc ((c00, ((ub c00 t r0 t2), (nonce 150))), TWO) (pke 11) (er 7)) in
                        let phi02':= [msg b00, msg b11, msg e00', msg e11] in
                        let fphi02':= f (toListm phi02') in
-                       let s0':= (If (! (isin pv00 ((pi1 (d 1 fphi02')), ((pi1 (d 2 fphi02')), (pi1 (d 3 fphi02')))))) then (shufl (pi1 (d 1 fphi02')) (pi1 (d 2 fphi02')) (pi1 (d 3 fphi02'))) else O)in
+                       let dd n s :=  If (tau n s) #? e00' then (d n s) else (d n s) in
+                       let s0':= (If (! (isin pv00 ((pi1 (dd 1 fphi02')), ((pi1 (dd 2 fphi02')), (pi1 (dd 3 fphi02')))))) then (shufl (pi1 (dd 1 fphi02')) (pi1 (dd 2 fphi02')) (pi1 (dd 3 fphi02'))) else O)in
                        let dv0' := (If (dist fphi02') & (pvchecks fphi02') then s0' else |_) in
                        let phi03':= phi02' ++[msg dv0'] in
                        let fphi03' := f (toListm phi03') in
@@ -158,13 +189,17 @@ Proof. intros.
                        let l11' := (If (bnlcheck c11 (nonce 21) fphi03') then (enc ((label c11 fphi03'), (k1, THREE)) (pke 11) (er 10)) else O) in
                        let phi05':= phi03'++[msg l00', msg l11'] in
                        let fphi05' := f (toListm phi05') in
-                       let do0' := (If (dist fphi05') & (pochecks fphi05') & (((isink k0 fphi05') & (isink k1 fphi05')))(* or (! ((isink k0 fphi05')or (isink k1 fphi05'))))*) then (sotrm fphi05') else |_) in
+                       let p' n x := ( (tau 1 (dd n x)), (tau 2 (dd n x))) in
+                       let sotrm' x := (shufl (p' 1 x) (p' 2 x) (p' 3 x)) in
+                       let do0' := (If (dist fphi05') & (pochecks fphi05') & (((isink k0 fphi05') & (isink k1 fphi05')))(* or (! ((isink k0 fphi05')or (isink k1 fphi05'))))*) then (sotrm' fphi05') else |_) in
                        let t0s0' := (If acc00 & acc11 then ((e00', (e11, dv0')), (l00', (l11', do0'))) else |_) in
                        [msg b00, msg b11, msg t0s0'])
-                       (let e10' := (enc ((c10, ((ub c10 t r0 t4), (nonce 150))), TWO) (pke 11) (er 7)) in
+
+                      (let e10' := (enc ((c10, ((ub c10 t r0 t4), (nonce 150))), TWO) (pke 11) (er 7)) in
                         let phi12':= [msg b10, msg b01, msg e10', msg e01] in
                         let fphi12':= f (toListm phi12') in
-                        let s1' := (If (! (isin pv10 ((pi1 (d 1 fphi12')), ((pi1 (d 2 fphi12')), (pi1 (d 3 fphi12')))))) then (shufl (pi1 (d 1 fphi12')) (pi1 (d 2 fphi12')) (pi1 (d 3 fphi12'))) else O)in
+                        let dd n s :=  If (tau n s) #? e10' then (d n s) else (d n s) in
+                        let s1' := (If (! (isin pv10 ((pi1 (dd 1 fphi12')), ((pi1 (dd 2 fphi12')), (pi1 (dd 3 fphi12')))))) then (shufl (pi1 (dd 1 fphi12')) (pi1 (dd 2 fphi12')) (pi1 (dd 3 fphi12'))) else O)in
                         let dv1' := (If (dist fphi12') & (pvchecks fphi12') then s1' else |_) in
                         let phi13':= phi12' ++[msg dv1'] in
                         let fphi13' := f (toListm phi13') in
@@ -172,12 +207,95 @@ Proof. intros.
                         let l01' := (If (bnlcheck c01 (nonce 21) fphi13') then (enc ((label c01 fphi13'), (k1, THREE)) (pke 11) (er 10)) else O) in
                         let phi15':= phi13'++[msg l10', msg l01'] in
                         let fphi15' := f (toListm phi15') in
-                        let do1' := (If (dist fphi15')& (pochecks fphi15')& (((isink k0 fphi15')&(isink k1 fphi15'))) (*or (! ((isink k0 fphi15')or (isink k1 fphi15'))))*) then (sotrm fphi15') else |_) in
+                        let p' n x := ( (tau 1 (dd n x)), (tau 2 (dd n x))) in
+                        let sotrm' x := (shufl (p' 1 x) (p' 2 x) (p' 3 x)) in
+                        let do1' := (If (dist fphi15')& (pochecks fphi15')& (((isink k0 fphi15')&(isink k1 fphi15'))) (*or (! ((isink k0 fphi15')or (isink k1 fphi15'))))*) then (sotrm' fphi15') else |_) in
                         let t1s1' := (If acc10 & acc01 then ((e10', (e01, dv1')), (l10', (l01', do1'))) else |_) in
-                        [msg b10, msg b01, msg t1s1']).
+                          [msg b10, msg b01, msg t1s1']).
+       Ltac rewDecs t n x n1 := rewrite <- (@IFSAME_M (t #? x) (dec t (ske n))) at n1.
+       (* assert (forall n: nat, d n fphi02 # If (tau n fphi02) #? e00 then (pv00, TWO) else (If (tau n fphi02) #? e11 then (pv11, TWO) else (d n fphi02))). *)
+       assert(forall (n:nat) (s:message), d n s # If (tau n s) #? e00 then (d n s) else (d n s)).
+       intros.
+       rewrite <- IFSAME_M with (b:= (tau n s) #? e00) at 1.
+       reflexivity.
+       unfold t0s0.
+       (* rewrite left-side *)
+       (* 2. rewrite decryptions in the opening phase  *)
+       unfold do0, sotrm, p.
+       Set Nested Proofs Allowed.
+       Add Parametric Morphism n: (@tau n) with
+           signature EQm ==> EQm as tau_mor.
+       Proof. intros; aply_cong; try auto. Qed.
+       rewrite H0 with (n:= 1) (s:= fphi05).
+       rewrite H0 with (n:= 2) (s:= fphi05).
+       rewrite H0 with (n:= 3) (s:= fphi05).
+       (* 1. rewrite the decryptions in voting phase *)
+       repeat unfold dv0, s0, l00, l11, do0, sotrm, p, fphi05, phi05, fphi03, phi03.
+        rewrite H0 with (n:= 1) (s:= fphi02).
+       rewrite H0 with (n:= 2) (s:= fphi02).
+       rewrite H0 with (n:= 3) (s:= fphi02).
 
-       (* replace nonce in the encryption term of the left frame using CCA2, L ~ L'  *)
-       Axiom ENCCCA2: forall (n n1 n2 n3: nat) (u u': message) {m} (l: mylist m),
+       (* Apply CCA2 definition using context *)
+       pose proof (@cca2CxtAxiom 11 7 7 (pv00, TWO) ((c00, ((ub c00 t r0 t2), (nonce 150))), TWO)
+                            (fun x => let e00' := x in
+                                      let phi02':= [msg b00, msg b11, msg e00', msg e11] in
+                                      let fphi02':= f (toListm phi02') in
+                                      let dd n s :=  If (tau n s) #? e00 then (d n s) else (d n s) in
+                             let s0':= (If (! (isin pv00 ((pi1 (dd 1 fphi02')), ((pi1 (dd 2 fphi02')), (pi1 (dd 3 fphi02')))))) then (shufl (pi1 (dd 1 fphi02')) (pi1 (dd 2 fphi02')) (pi1 (dd 3 fphi02'))) else O)in
+                             let dv0' := (If (dist fphi02') & (pvchecks fphi02') then s0' else |_) in
+                             let phi03':= phi02' ++[msg dv0'] in
+                             let fphi03' := f (toListm phi03') in
+                             let l00' := (If (bnlcheck c00 (nonce 20) fphi03') then (enc ((label c00 fphi03'), (k0, THREE)) (pke 11) (er 9)) else O) in
+                             let l11' := (If (bnlcheck c11 (nonce 21) fphi03') then (enc ((label c11 fphi03'), (k1, THREE)) (pke 11) (er 10)) else O) in
+                             let phi05':= phi03'++[msg l00', msg l11'] in
+                             let fphi05' := f (toListm phi05') in
+                             let p' n x := ( (tau 1 (dd n x)), (tau 2 (dd n x))) in
+                             let sotrm' x := (shufl (p' 1 x) (p' 2 x) (p' 3 x)) in                                                     let do0' := (If (dist fphi05') & (pochecks fphi05') & (((isink k0 fphi05') & (isink k1 fphi05')))(* or (! ((isink k0 fphi05')or (isink k1 fphi05'))))*) then (sotrm' fphi05') else |_) in
+                                                                                                                                       let t0s0' := (If acc00 & acc11 then ((e00', (e11, dv0')), (l00', (l11', do0'))) else |_) in
+                                                                                                                                       [msg b00; msg b11; msg t0s0'])). simpl in H1. apply H1.
+   msg
+     (If (f [b00; b11; x]) #? x
+         then (pv00, TWO)
+      else dec (f [b00; b11; x]) (ske 11))])).
+       rewr       (
+       rewrite H0 with (n:= 1) (s:= (f (toListm [msg b00, msg b11, msg (enc ((c00, ((ub c00 t r0 t2), (nonce 150))), TWO) (pke 11) (er 7)), msg e11]))).
+
+       rewrite <- (@IFSAME_M ((tau n fphi02) #? e11) (dec (tau n fphi02) (ske 11))) at 2.
+       (** This should be proved using EQBRANCH *)
+       Axiom rewEqBrDec: forall m1 m2 m3 m4: message, (If m1 #? m2 then dec m1 m3 else m4) # (If m1 #? m2 then (dec m2 m3) else m4).
+       repeat rewrite rewEqBrDec.
+       reflexivity.
+
+       apply (@cca2CxtAxiom 11 7 7 (pv00, TWO) (pv00, TWO) (fun x => [msg b00; msg b11; msg x;
+   msg
+     (If (f [b00; b11; x]) #? x
+         then (pv00, TWO)
+      else dec (f [b00; b11; x]) (ske 11))])).
+
+       Focus 2. constructor. unfold b00. repeat constructor. repeat constructor. Focus 2. reflexivity.      Focus 2. reflexivity. Focus 2. simpl. reflexivity.  apply len_reg. repeat apply eqmeql.
+       apply eqmeql.
+       assert (s0 # s0).
+       unfold s0. unfold d.
+       Set Nested Proofs Allowed.
+
+       rewDecs (tau 1 fphi02) 11 e00 ((c00, ((ub c00 t r0 t2), (nonce 150))), TWO) ((c00, ((ub c00 t r0 t2), (nonce 150))), TWO).
+
+       (* replace nonce in the encryption term of the left frame using CCA2, L ~ L' *)
+       (* Axiom rewDecryption: forall n x e, dec x (ske n) # If x #? e then O else (dec x (ske n)). *)
+       Fixpoint rewDecs n x (l: Mlist) : message :=
+         match l with
+         | [ ] => dec x (ske n)
+         | h :: t => If x #? h then O else rewDecs n x t
+         end.
+       Axiom rewDecryption: forall n x l, dec x (ske n) # (rewDecs n x l).
+
+       Ltac rewDecs n listEncs :=
+       match goal with
+       |[|- context[dec ?X (ske n)] ] => rewrite (@rewDecryption n X listEncs)
+       end.
+          match listEncs
+       rewrite (@rewDecryption 11).
+                       Axiom ENCCCA2: forall (n n1 n2 n3: nat) (u u': message) {m} (l: mylist m),
     (|u|#?|u'|) ## TRue ->
     (List.length (distMvars l) <=? 1) = true ->
     distMvars l = (cons n nil) ->
@@ -199,11 +317,11 @@ Proof. intros.
                             let t0s0' := (If acc00 & acc11 then ((e00', (e11, dv0')), (l00', (l11', do0'))) else |_) in
                             [msg b00, msg b11, msg t0s0'])) as cca2.
 
-       
 
-        simpl in cca2.
+
+         simpl in cca2.
                            If (acc00) & acc11
-        then (e00', (e11, dv0'), (l00', (l11', do0'))) 
+        then (e00', (e11, dv0'), (l00', (l11', do0')))
         else |_ in
    [msg b00, msg b11, msg t0s0']
        simpl in H0.
@@ -222,16 +340,16 @@ Proof. intros.
        funapp_f3m_in shufl 7 6 5 H0.
        funapp_fm_in O H0.
        funapp_f3bm_in ifm_then_else_ 3 2 1 H0.
-     
+
        tacFuncAppFmb pvchecks 23 H0.
        tacFuncAppFmb dist 24 H0.
        funapp_andB_in 1 2 H0.
        funapp_fm_in |_ H0.
        funapp_f3bm_in ifm_then_else_ 2 5 1 H0.
        tacFuncAppAttComp' [21; 22; 27; 26; 1] H0.
-     
+
        tacFunAppNatMsg nonce 20 H0.
-       
+
        funapp_f3mb_in bnlcheck 21 1 2 H0.
        tacFunAppNatMsg nonce 21 H0.
        funapp_f3mb_in bnlcheck 24 1 4 H0.
@@ -257,7 +375,7 @@ Proof. intros.
        tacFunAppNatMsg er 9 H0.
        funapp_f3m_in enc 3 2 1 H0.
        restr_proj_in 2 H0.
-       restr_proj_in 3 H0. 
+       restr_proj_in 3 H0.
        tacFunAppNatMsg er 10 H0.
        funapp_f3m_in enc 4 3 1 H0.
        restr_proj_in 5 H0.
@@ -266,20 +384,20 @@ Proof. intros.
        restr_proj_in 6 H0.
        restr_proj_in 8 H0.
        funapp_fm_in O H0.
-       funapp_f3bm_in ifm_then_else_ 6 2 1 H0. 
+       funapp_f3bm_in ifm_then_else_ 6 2 1 H0.
        do 2 restr_proj_in 2 H0.
-       restr_proj_in 5 H0. 
+       restr_proj_in 5 H0.
        restr_proj_in 6 H0.
        funapp_fm_in O H0.
        funapp_f3bm_in ifm_then_else_ 6 3 1 H0.
        restr_proj_in 2 H0.
        restr_proj_in 3 H0.
-       restr_proj_in 5 H0. 
+       restr_proj_in 5 H0.
        do 18 restr_proj_in 6 H0.
-       chkType H0. 
+       chkType H0.
        tacFuncAppAttComp' [7;8; 13; 12; 5; 1; 2] H0.
        tacFuncAppFmb dist 1 H0.
-       tacFuncAppFmb pochecks 2 H0. 
+       tacFuncAppFmb pochecks 2 H0.
        funapp_f2b_in isin 7 3 H0.
        funapp_f2b_in isin 7 4 H0.
        funapp_andB_in 4 3 H0.
@@ -290,7 +408,7 @@ Proof. intros.
        do 4 restr_proj_in 2 H0.
        funapp_f1_in sotrm 2 H0.
        restr_proj_in 3 H0.
-       funapp_fm_in |_ H0. 
+       funapp_fm_in |_ H0.
        funapp_f3bm_in ifm_then_else_ 3 2 1 H0.
        do 3 restr_proj_in 2 H0.
        chkType H0.
@@ -304,7 +422,7 @@ Proof. intros.
        restr_proj_in 3 H0.
        funapp_f2m_in pair 2 1 H0.
        do 2 restr_proj_in 2 H0.
-       chkType H0.  
+       chkType H0.
        funapp_f2m_in pair 6 2 H0.
          funapp_f2m_in pair 8 1 H0.
        restr_proj_in 2 H0.
@@ -313,12 +431,13 @@ Proof. intros.
        funapp_fm_in |_ H0.
        funapp_f3bm_in ifm_then_else_ 5 2 1 H0.
        restrsublis H0; try auto.
-       repeat (try apply len_reg; try rewrite eqmeql; try apply nameEql; try simpl; try intuition).
+       repeat (try apply len_reg; try rewrite eqmeql; try apply nameEql; try simpl; try intuition).*)
        (* ********************* *)
        (* replace nonce in the encryption term of the right frame using CCA2, R ~ R'  *)
        (* ************************ *)
-       split. 
-       pose proof (let n1:= 11 in
+       split.
+       apply dummy.
+(*       pose proof (let n1:= 11 in
                    let n2:= 7 in
                    let n3:= 7 in
                    let u:= (c10, (ub c10 t r0 t4, nonce 20), TWO) in
@@ -341,16 +460,16 @@ Proof. intros.
        funapp_f3m_in shufl 7 6 5 H0.
        funapp_fm_in O H0.
        funapp_f3bm_in ifm_then_else_ 3 2 1 H0.
-     
+
        tacFuncAppFmb pvchecks 23 H0.
        tacFuncAppFmb dist 24 H0.
        funapp_andB_in 1 2 H0.
        funapp_fm_in |_ H0.
        funapp_f3bm_in ifm_then_else_ 2 5 1 H0.
        tacFuncAppAttComp' [21; 22; 27; 26; 1] H0.
-     
+
        tacFunAppNatMsg nonce 20 H0.
-       
+
        funapp_f3mb_in bnlcheck 21 1 2 H0.
        tacFunAppNatMsg nonce 21 H0.
        funapp_f3mb_in bnlcheck 24 1 4 H0.
@@ -376,7 +495,7 @@ Proof. intros.
        tacFunAppNatMsg er 9 H0.
        funapp_f3m_in enc 3 2 1 H0.
        restr_proj_in 2 H0.
-       restr_proj_in 3 H0. 
+       restr_proj_in 3 H0.
        tacFunAppNatMsg er 10 H0.
        funapp_f3m_in enc 4 3 1 H0.
        restr_proj_in 5 H0.
@@ -385,20 +504,20 @@ Proof. intros.
        restr_proj_in 6 H0.
        restr_proj_in 8 H0.
        funapp_fm_in O H0.
-       funapp_f3bm_in ifm_then_else_ 6 2 1 H0. 
+       funapp_f3bm_in ifm_then_else_ 6 2 1 H0.
        do 2 restr_proj_in 2 H0.
-       restr_proj_in 5 H0. 
+       restr_proj_in 5 H0.
        restr_proj_in 6 H0.
        funapp_fm_in O H0.
        funapp_f3bm_in ifm_then_else_ 6 3 1 H0.
        restr_proj_in 2 H0.
        restr_proj_in 3 H0.
-       restr_proj_in 5 H0. 
+       restr_proj_in 5 H0.
        do 18 restr_proj_in 6 H0.
-       chkType H0. 
+       chkType H0.
        tacFuncAppAttComp' [7;8; 13; 12; 5; 1; 2] H0.
        tacFuncAppFmb dist 1 H0.
-       tacFuncAppFmb pochecks 2 H0. 
+       tacFuncAppFmb pochecks 2 H0.
        funapp_f2b_in isin 7 3 H0.
        funapp_f2b_in isin 7 4 H0.
        funapp_andB_in 4 3 H0.
@@ -409,7 +528,7 @@ Proof. intros.
        do 4 restr_proj_in 2 H0.
        funapp_f1_in sotrm 2 H0.
        restr_proj_in 3 H0.
-       funapp_fm_in |_ H0. 
+       funapp_fm_in |_ H0.
        funapp_f3bm_in ifm_then_else_ 3 2 1 H0.
        do 3 restr_proj_in 2 H0.
        chkType H0.
@@ -423,7 +542,7 @@ Proof. intros.
        restr_proj_in 3 H0.
        funapp_f2m_in pair 2 1 H0.
        do 2 restr_proj_in 2 H0.
-       chkType H0.  
+       chkType H0.
        funapp_f2m_in pair 6 2 H0.
          funapp_f2m_in pair 8 1 H0.
        restr_proj_in 2 H0.
@@ -529,7 +648,7 @@ apply funcAppRestr with (p1:=0) (p2:=1) (f:= (fun x y =>
                                                          else |_ in
                                                          [msg b10, msg b01, msg t1s1'])) in cca2.
        simpl in cca2.
-       apply cca2.  repeat (try apply len_reg; try rewrite eqmeql; try apply nameEql; simpl; intuition). auto.
+       apply cca2.  repeat (try apply len_reg; try rewrite eqmeql; try apply nameEql; simpl; intuition). auto.*)
        (* ********************************** *)
        (*   *********************************************************** *)
        (*   Done replacing nonce 20 using CCA2  *)
@@ -569,8 +688,8 @@ apply funcAppRestr with (p1:=0) (p2:=1) (f:= (fun x y =>
                 | [|- context [ _ or FAlse ] ] => rewrite orB_FAlse_r
                 end; redg.
        rewOrBFalse.
-       pose proof(compHid 3 4 v0 v1 []) as ch. simpl in ch. simpl.
-       apply funcAppRestrCompHid with (n1:= 3) (n2:=4) (v0:= v0) (v1:= v1) (f:= fun x y => let b00 := (bl x t r0) in
+       pose proof(compHid 3 4 v0 v1 []) as ch. simpl in ch.
+       (*apply funcAppRestrCompHid with (n1:= 3) (n2:=4) (v0:= v0) (v1:= v1) (f:= fun x y => let b00 := (bl x t r0) in
                                                  let b11 := (bl y t r1) in
                                                  let t0 := (((vk 0), (Mvar 5), sign (Mvar 5) (ssk 0) (sr 14)), ((vk 1), (Mvar 6), sign (Mvar 6) (ssk 1) (sr 15))) in
                                                  let t1 := (t0, f (cons t0 nil)) in
@@ -584,7 +703,7 @@ apply funcAppRestr with (p1:=0) (p2:=1) (f:= (fun x y =>
                                                  let pv11 := (y, ((ub y t r1 t3), (nonce 21))) in
                                                  let phi02':= [msg b00, msg b11, msg e00', msg e11] in
                                                  let fphi02':= f (toListm phi02') in
-                                                 [msg b00, msg b11, msg (If (acc00) & acc11
+                                                 [msg b00; msg b11; msg (If (acc00) & acc11
                                                                          then (e00', (e11,
                                                                                        If (dist (f [b00; b11; e00'; e11])) & (pvchecks (f [b00; b11; e00'; e11]))
                                                                                       then
@@ -597,10 +716,14 @@ apply funcAppRestr with (p1:=0) (p2:=1) (f:= (fun x y =>
                                                        else (bnlcheck y (nonce 21) (f [b00; b11; e00'; e11; |_]))) then
                                                      (enc ( If (dist (f [b00; b11; e00'; e11])) & (pvchecks (f [b00; b11; e00'; e11]))
                                                                                       then
-                                                                                        (If (! (isin pv00 ((pi1 (d 1 fphi02')), ((pi1 (d 2 fphi02')), (pi1 (d 3 fphi02')))))) then  (label y (f [b00; b11; e00'; e11; (shufl (pi1 (d 1 fphi02')) (pi1 (d 2 fphi02')) (pi1 (d 3 fphi02')))])) else (label y (f [b00; b11; e00'; e11; O]))) else (label y (f [b00; b11; e00'; e11; |_])), (k1, THREE)) (pke 11) (er 10)) else O, |_))) else |_)]) in ch.
+                                                                                        (If (! (isin pv00 ((pi1 (d 1 fphi02')), ((pi1 (d 2 fphi02')), (pi1 (d 3 fphi02')))))) then  (label y (f [b00; b11; e00'; e11; (shufl (pi1 (d 1 fphi02')) (pi1 (d 2 fphi02')) (pi1 (d 3 fphi02')))])) else (label y (f [b00; b11; e00'; e11; O]))) else (label y (f [b00; b11; e00'; e11; |_])), (k1, THREE)) (pke 11) (er 10)) else O, |_))) else |_)]) in ch. *)
  simpl in ch.
+      Focus 4. constructor.
+repeat constructor. simpl.
 
-                            apply ch. repeat try split; simpl; try apply vchecksImplyVoteEql. auto.
+       Focus 4.
+
+       apply ch. repeat try split; simpl; try apply vchecksImplyVoteEql. auto.
 
 Qed.
 
