src/voteprivacy/newCca2Compliant.v
@@ -1,0 +1,90 @@
+Require Export contextCompHid.
+Import ListNotations.
+
+Module newCca2Compliant.
+Search eq.
+
+Inductive Cca2CxtMsg (n n1: nat) (u u': message): message ->  Prop :=
+| Cnonce (n2 : nat): beq_nat n n2 = false -> Cca2CxtMsg n n1 u u' (nonce n2)
+| CVar n2: n2 = n1 -> Cca2CxtMsg n n1 u u' (Mvar n2) 
+| CO: Cca2CxtMsg n n1 u u' O
+| Cpair t1 t2 (H1: Cca2CxtMsg n n1 u u' t1) (H2: Cca2CxtMsg n n1 u u' t2): Cca2CxtMsg n n1 u u' (pair t1 t2)
+| Cifm_then_else_ b t1 t2 (H1: Cca2CxtBol n n1 u u' b) (H2: Cca2CxtMsg n n1 u u' t1) (H3: Cca2CxtMsg n n1 u u' t2): Cca2CxtMsg n n1 u u' (ifm_then_else_ b t1 t2)
+(*| rewDec C1 C2 (H1: Cca2CxtMsg n C1) (H2: Cca2CxtMsg n C2): Cca2CxtMsg n (fun (x: message) => If ((C1 x) #? x) then (C2 x) else (dec (C1 x) (ske n)))*)
+| Cpi1 t1 (H1: Cca2CxtMsg n n1 u u' t1): Cca2CxtMsg n n1 u u' t1
+| Cpi2 t1 (H1: Cca2CxtMsg n n1 u u' t1): Cca2CxtMsg n n1 u u' t1
+| Cto t1 (H1: Cca2CxtMsg n n1 u u' t1): Cca2CxtMsg n n1 u u' t1
+| CL t1 (H1: Cca2CxtMsg n n1 u u' t1): Cca2CxtMsg n n1 u u' t1
+| Cf L (H1: Cca2CxtListMsg n n1 u u' L): Cca2CxtMsg n n1 u u' (f L) 
+| CONE: Cca2CxtMsg n n1 u u' ONE
+| CTWO: Cca2CxtMsg n n1 u u' TWO
+| CTHREE: Cca2CxtMsg n n1 u u' THREE
+| CA: Cca2CxtMsg n n1 u u' A 
+| CB: Cca2CxtMsg n n1 u u' B
+| CM: Cca2CxtMsg n n1 u u' M
+| CC1: Cca2CxtMsg n n1 u u' C1
+| CC2: Cca2CxtMsg n n1 u u' C2
+| CC3: Cca2CxtMsg n n1 u u' C3
+| CV0 C1 (H1: Cca2CxtMsg n n1 u u' C1): Cca2CxtMsg n n1 u u' (V0 C1)
+| CV1 C1 (H1: Cca2CxtMsg n n1 u u' C1): Cca2CxtMsg n n1 u u' (V1 C1)
+| Cpubkey C1 (H1: Cca2CxtMsg n n1 u u' C1): Cca2CxtMsg n n1 u u' (pubkey C1)
+(* Commitments *)
+| Ckc C1 (H1: Cca2CxtMsg n n1 u u' C1): Cca2CxtMsg n n1 u u' (kc C1)
+| Ccomm C1 C2 (H1: Cca2CxtMsg n n1 u u' C1) (H2: Cca2CxtMsg n n1 u u' C2):
+  Cca2CxtMsg n n1 u u' (comm C1 C2)
+| Copen C1 C2 C3 (H1: Cca2CxtMsg n n1 u u' C1) (H2: Cca2CxtMsg n n1 u u' C2) (H3: Cca2CxtMsg n n1 u u' C3):
+  Cca2CxtMsg n n1 u u' (open C1 C2 C3)
+(* shuffling *)
+| Cshufle C1 C2 C3 (H1: Cca2CxtMsg n n1 u u' C1) (H2: Cca2CxtMsg n n1 u u' C2) (H3: Cca2CxtMsg n n1 u u' C3):
+  Cca2CxtMsg n n1 u u' (shufl C1 C2 C3)
+(* Encryptions  *)
+| Cke C1 (H1: Cca2CxtMsg n n1 u u' C1): Cca2CxtMsg n n1 u u' (ke C1)
+| Cre C1 (H1: Cca2CxtMsg n n1 u u' C1): Cca2CxtMsg n n1 u u' (re C1)
+| Cenc C1 C2 C3 (H1: Cca2CxtMsg n n1 u u' C1) (H2: Cca2CxtMsg n n1 u u' C2) (H3: Cca2CxtMsg n n1 u u' C3): Cca2CxtMsg n n1 u u' (enc C1 C2 C3)
+| Cdect C1 C2 n2 (H1: Cca2CxtMsg n n1 u u' C1) :  beq_nat n2 n = true  -> Cca2CxtMsg n n1 u u' (If (C1 #? (Mvar n1)) then C2 else (dec C1 (ske n2)))
+| Cdecf C1 n2 (H1: Cca2CxtMsg n n1 u u' C1) :  beq_nat n2 n = false  -> Cca2CxtMsg n n1 u u' (dec C1 (ske n2))
+(*   Cca2CxtMsg n n1 u u' *)
+(* Blind signatures *)
+| Cbot : Cca2CxtMsg n n1 u u' bot 
+| Ckb C1 (H1: Cca2CxtMsg n n1 u u' C1): Cca2CxtMsg n n1 u u' (kb C1)
+| Crb C1 (H1: Cca2CxtMsg n n1 u u' C1): Cca2CxtMsg n n1 u u' (rb C1)
+| Cbsign C1 C2 C3 (H1: Cca2CxtMsg n n1 u u' C1) (H2: Cca2CxtMsg n n1 u u' C2) (H3: Cca2CxtMsg n n1 u u' C3): Cca2CxtMsg n n1 u u' (bsign C1 C2 C3)
+| Cbl C1 C2 C3 (H1: Cca2CxtMsg n n1 u u' C1) (H2: Cca2CxtMsg n n1 u u' C2) (H3: Cca2CxtMsg n n1 u u' C3): Cca2CxtMsg n n1 u u' (bl C1 C2 C3)
+| Cub C1 C2 C3 C4 (H1: Cca2CxtMsg n n1 u u' C1) (H2: Cca2CxtMsg n n1 u u' C2) (H3: Cca2CxtMsg n n1 u u' C3) (H4: Cca2CxtMsg n n1 u u' C4):
+  Cca2CxtMsg n n1 u u' (ub C1 C2 C3 C4)
+(* Signatures *)
+| Cks C1 (H1: Cca2CxtMsg n n1 u u' C1): Cca2CxtMsg n n1 u u' (ks C1)
+| Crs C1 (H1: Cca2CxtMsg n n1 u u' C1): Cca2CxtMsg n n1 u u' (rs C1)
+| Csign C1 C2 C3 (H1: Cca2CxtMsg n n1 u u' C1) (H2: Cca2CxtMsg n n1 u u' C2) (H3: Cca2CxtMsg n n1 u u' C3): Cca2CxtMsg n n1 u u' (sign C1 C2 C3)
+(* Zero symbol  *)
+| Cz C1 (H1: Cca2CxtMsg n n1 u u' C1): Cca2CxtMsg n n1 u u' (z C1)
+(* Compl symbol *)
+| Ccompl C1 (H1: Cca2CxtMsg n n1 u u' C1): Cca2CxtMsg n n1 u u' (compl C1)
+with
+  Cca2CxtBol (n n1: nat) (u u': message) : Bool -> Prop :=
+| CTRue: Cca2CxtBol n n1 u u' TRue
+| CFAlse: Cca2CxtBol n n1 u u' FAlse
+| Ceqb C1 C2 (H1: Cca2CxtBol n n1 u u' C1) (H2: Cca2CxtBol n n1 u u' C2): Cca2CxtBol n n1 u u' (eqb C1 C2)
+| Ceqm C1 C2 (H1: Cca2CxtMsg n n1 u u' C1) (H2: Cca2CxtMsg n n1 u u' C2): Cca2CxtBol n n1 u u' (eqm C1 C2)
+| Cifb_then_else_ C1 C2 C3 (H1: Cca2CxtBol n n1 u u' C1) (H2: Cca2CxtBol n n1 u u' C2) (H3: Cca2CxtBol n n1 u u' C3):
+  Cca2CxtBol n n1 u u' (ifb_then_else_ C1 C2 C3)         
+| Cacc C1 C2 C3 C4 (H1: Cca2CxtMsg n n1 u u' C1) (H2: Cca2CxtMsg n n1 u u' C2) (H3: Cca2CxtMsg n n1 u u' C3) (H4: Cca2CxtMsg n n1 u u' C4):
+  Cca2CxtBol n n1 u u' (acc C1 C2 C3 C4)
+| Cbver C1 C2 C3 (H1: Cca2CxtMsg n n1 u u' C1) (H2: Cca2CxtMsg n n1 u u' C2) (H3: Cca2CxtMsg n n1 u u' C3):
+  Cca2CxtBol n n1 u u' (bver C1 C2 C3)
+| Cver C1 C2 C3 (H1: Cca2CxtMsg n n1 u u' C1) (H2: Cca2CxtMsg n n1 u u' C2) (H3: Cca2CxtMsg n n1 u u' C3):
+  Cca2CxtBol n n1 u u' (ver C1 C2 C3)
+with
+  Cca2CxtListMsg (n n1: nat) (u u': message): list message -> Prop:=
+| CNil: Cca2CxtListMsg n n1 u u' [ ]
+| CCons C L (H1:Cca2CxtMsg n n1 u u' C) (H2:Cca2CxtListMsg n n1 u u' L): Cca2CxtListMsg n n1 u u' (C :: L).
+End newCca2Compliant.
+Import newCca2Compliant.
+Axiom ENCCCA2: forall (n n1 n2 n3: nat) (u u': message) {m} (l: mylist m),
+    (|u|#?|u'|) ## TRue ->
+    (List.length (distMvars l) <=? 1) = true ->
+    distMvars l = (cons n nil) ->
+    (closMylist [msg u, msg u'] = true) ->
+    Cca2CxtListMsg n1 n u u' (toListm l) ->
+    ([ n <- {u}_n1^^n2 ] l) ~ ([ n <- {u'}_n1^^n3] l).
+                            
